<?xml version="1.0"?>
<rdf:RDF xmlns="http://www.semanticweb.org/team3/robo-ontology-0#"
     xml:base="http://www.semanticweb.org/team3/robo-ontology-0"
     xmlns:owl="http://www.w3.org/2002/07/owl#"
     xmlns:rdf="http://www.w3.org/1999/02/22-rdf-syntax-ns#"
     xmlns:xml="http://www.w3.org/XML/1998/namespace"
     xmlns:xsd="http://www.w3.org/2001/XMLSchema#"
     xmlns:rdfs="http://www.w3.org/2000/01/rdf-schema#">
    <owl:Ontology rdf:about="http://www.semanticweb.org/team3/robo-ontology-0"/>
    


    <!-- 
    ///////////////////////////////////////////////////////////////////////////////////////
    //
    // Annotation properties
    //
    ///////////////////////////////////////////////////////////////////////////////////////
     -->

    


    <!-- http://www.w3.org/2000/01/rdf-schema#near -->

    <owl:AnnotationProperty rdf:about="http://www.w3.org/2000/01/rdf-schema#near"/>
    


    <!-- 
    ///////////////////////////////////////////////////////////////////////////////////////
    //
    // Object Properties
    //
    ///////////////////////////////////////////////////////////////////////////////////////
     -->

    


    <!-- http://www.semanticweb.org/team3/robo-ontology-0#OWLObjectProperty_a86449e2_fff3_4ffd_8434_7e4502187135 -->

    <owl:ObjectProperty rdf:about="http://www.semanticweb.org/team3/robo-ontology-0#OWLObjectProperty_a86449e2_fff3_4ffd_8434_7e4502187135">
        <rdfs:domain rdf:resource="http://www.semanticweb.org/team3/robo-ontology-0#Object"/>
        <rdfs:label xml:lang="en">valueNear</rdfs:label>
    </owl:ObjectProperty>
    


    <!-- http://www.semanticweb.org/team3/robo-ontology-0#hasMethod -->

    <owl:ObjectProperty rdf:about="http://www.semanticweb.org/team3/robo-ontology-0#hasMethod">
        <rdfs:domain rdf:resource="http://www.semanticweb.org/team3/robo-ontology-0#Robo"/>
        <rdfs:range rdf:resource="http://www.semanticweb.org/team3/robo-ontology-0#Method"/>
        <rdfs:label xml:lang="en">hasMethod</rdfs:label>
    </owl:ObjectProperty>
    


    <!-- http://www.semanticweb.org/team3/robo-ontology-0#hasParameter -->

    <owl:ObjectProperty rdf:about="http://www.semanticweb.org/team3/robo-ontology-0#hasParameter">
        <rdfs:domain rdf:resource="http://www.semanticweb.org/team3/robo-ontology-0#Method"/>
        <rdfs:range rdf:resource="http://www.semanticweb.org/team3/robo-ontology-0#Parameter"/>
        <rdfs:label xml:lang="en">hasParameter</rdfs:label>
    </owl:ObjectProperty>
    


    <!-- http://www.semanticweb.org/team3/robo-ontology-0#hasValue -->

    <owl:ObjectProperty rdf:about="http://www.semanticweb.org/team3/robo-ontology-0#hasValue">
        <rdfs:domain rdf:resource="http://www.semanticweb.org/team3/robo-ontology-0#DataType"/>
        <rdfs:range rdf:resource="http://www.semanticweb.org/team3/robo-ontology-0#Value"/>
        <rdfs:label rdf:datatype="http://www.w3.org/2001/XMLSchema#string">hasValue</rdfs:label>
    </owl:ObjectProperty>
    


    <!-- http://www.semanticweb.org/team3/robo-ontology-0#ofDataType -->

    <owl:ObjectProperty rdf:about="http://www.semanticweb.org/team3/robo-ontology-0#ofDataType">
        <rdfs:domain rdf:resource="http://www.semanticweb.org/team3/robo-ontology-0#Parameter"/>
        <rdfs:range rdf:resource="http://www.semanticweb.org/team3/robo-ontology-0#DataType"/>
        <rdfs:label xml:lang="en">ofDataType</rdfs:label>
    </owl:ObjectProperty>
    


    <!-- 
    ///////////////////////////////////////////////////////////////////////////////////////
    //
    // Data properties
    //
    ///////////////////////////////////////////////////////////////////////////////////////
     -->

    


    <!-- http://www.semanticweb.org/team3/robo-ontology-0#closeDistance -->

    <owl:DatatypeProperty rdf:about="http://www.semanticweb.org/team3/robo-ontology-0#closeDistance">
        <rdfs:domain rdf:resource="http://www.semanticweb.org/team3/robo-ontology-0#Object"/>
        <rdfs:range rdf:resource="http://www.w3.org/2001/XMLSchema#double"/>
        <rdfs:label xml:lang="en">closeDistance</rdfs:label>
    </owl:DatatypeProperty>
    


    <!-- http://www.semanticweb.org/team3/robo-ontology-0#farDistance -->

    <owl:DatatypeProperty rdf:about="http://www.semanticweb.org/team3/robo-ontology-0#farDistance">
        <rdfs:label xml:lang="en">farDistance</rdfs:label>
    </owl:DatatypeProperty>
    


    <!-- http://www.semanticweb.org/team3/robo-ontology-0#midDistance -->

    <owl:DatatypeProperty rdf:about="http://www.semanticweb.org/team3/robo-ontology-0#midDistance">
        <rdfs:label xml:lang="en">midDistance</rdfs:label>
    </owl:DatatypeProperty>
    


    <!-- 
    ///////////////////////////////////////////////////////////////////////////////////////
    //
    // Classes
    //
    ///////////////////////////////////////////////////////////////////////////////////////
     -->

    


    <!-- http://www.semanticweb.org/team3/robo-ontology-0#DataType -->

    <owl:Class rdf:about="http://www.semanticweb.org/team3/robo-ontology-0#DataType">
        <rdfs:label xml:lang="en">DataType</rdfs:label>
    </owl:Class>
    


    <!-- http://www.semanticweb.org/team3/robo-ontology-0#Method -->

    <owl:Class rdf:about="http://www.semanticweb.org/team3/robo-ontology-0#Method">
        <rdfs:label xml:lang="en">Method</rdfs:label>
    </owl:Class>
    


    <!-- http://www.semanticweb.org/team3/robo-ontology-0#Object -->

    <owl:Class rdf:about="http://www.semanticweb.org/team3/robo-ontology-0#Object"/>
    


    <!-- http://www.semanticweb.org/team3/robo-ontology-0#Parameter -->

    <owl:Class rdf:about="http://www.semanticweb.org/team3/robo-ontology-0#Parameter">
        <rdfs:label xml:lang="en">Parameter</rdfs:label>
    </owl:Class>
    


    <!-- http://www.semanticweb.org/team3/robo-ontology-0#Robo -->

    <owl:Class rdf:about="http://www.semanticweb.org/team3/robo-ontology-0#Robo"/>
    


    <!-- http://www.semanticweb.org/team3/robo-ontology-0#State -->

    <owl:Class rdf:about="http://www.semanticweb.org/team3/robo-ontology-0#State"/>
    


    <!-- http://www.semanticweb.org/team3/robo-ontology-0#Value -->

    <owl:Class rdf:about="http://www.semanticweb.org/team3/robo-ontology-0#Value">
        <rdfs:label xml:lang="en">Value</rdfs:label>
    </owl:Class>
    


    <!-- 
    ///////////////////////////////////////////////////////////////////////////////////////
    //
    // Individuals
    //
    ///////////////////////////////////////////////////////////////////////////////////////
     -->

    


    <!-- Optional[http://www.semanticweb.org/team3/robo-ontology-0]/#Color -->

    <owl:NamedIndividual rdf:about="Optional[http://www.semanticweb.org/team3/robo-ontology-0]/#Color">
        <rdf:type rdf:resource="http://www.semanticweb.org/team3/robo-ontology-0#DataType"/>
        <hasValue rdf:resource="Optional[http://www.semanticweb.org/team3/robo-ontology-0]/#black"/>
        <hasValue rdf:resource="Optional[http://www.semanticweb.org/team3/robo-ontology-0]/#blue"/>
        <hasValue rdf:resource="Optional[http://www.semanticweb.org/team3/robo-ontology-0]/#brown"/>
        <hasValue rdf:resource="Optional[http://www.semanticweb.org/team3/robo-ontology-0]/#green"/>
        <hasValue rdf:resource="Optional[http://www.semanticweb.org/team3/robo-ontology-0]/#red"/>
        <hasValue rdf:resource="Optional[http://www.semanticweb.org/team3/robo-ontology-0]/#white"/>
        <hasValue rdf:resource="Optional[http://www.semanticweb.org/team3/robo-ontology-0]/#yellow"/>
        <rdfs:comment xml:lang="synonym">Color: colouration,colour,vividness,semblance,color,gloss,coloration,coloring,colouring_material,colouring,coloring_material</rdfs:comment>
    </owl:NamedIndividual>
    


    <!-- Optional[http://www.semanticweb.org/team3/robo-ontology-0]/#ConditionCloseToObject_06ee274d_73d9_44b1_96a5_24f057423e55 -->

    <owl:NamedIndividual rdf:about="Optional[http://www.semanticweb.org/team3/robo-ontology-0]/#ConditionCloseToObject_06ee274d_73d9_44b1_96a5_24f057423e55">
        <rdf:type rdf:resource="http://www.semanticweb.org/team3/robo-ontology-0#Method"/>
        <hasParameter rdf:resource="Optional[http://www.semanticweb.org/team3/robo-ontology-0]/#object_8e5c825e_02b6_40bc_8b54_0f165afa4201"/>
        <rdfs:comment xml:lang="synonym">Close: airless,secretive,cheeseparing,unaired,tightlipped,confining,closelipped,tight,penny-pinching,nigh,faithful,close-fitting,stuffy,snug,skinny,near,close,closemouthed</rdfs:comment>
        <rdfs:comment xml:lang="callstatement">IsCloseToObjectCondition</rdfs:comment>
        <rdfs:comment xml:lang="importstatement">edu.kit.ipd.ev3.conditions.IsCloseToObjectCondition</rdfs:comment>
        <rdfs:label xml:lang="en">ConditionCloseToObject</rdfs:label>
    </owl:NamedIndividual>
    


    <!-- Optional[http://www.semanticweb.org/team3/robo-ontology-0]/#ConditionLineDetected_e61c6675_10b2_4088_a3dd_14eadb032abf -->

    <owl:NamedIndividual rdf:about="Optional[http://www.semanticweb.org/team3/robo-ontology-0]/#ConditionLineDetected_e61c6675_10b2_4088_a3dd_14eadb032abf">
        <rdf:type rdf:resource="http://www.semanticweb.org/team3/robo-ontology-0#Method"/>
        <rdfs:comment xml:lang="synonym">Detected:</rdfs:comment>
        <rdfs:comment xml:lang="synonym">Line: lineage,argument,occupation,channel,personal_credit_line,production_line,line_of_credit,logical_argument,credit_line,business_line,stock,cable,blood_line,line_of_work,strain,demarcation,telephone_circuit,assembly_line,line_of_merchandise,product_line,melody,line_of_business,personal_line_of_credit,contrast,crease,line_of_descent,job,communication_channel,note,furrow,ancestry,billet,line_of_reasoning,line,railway_line,origin,seam,air,bloodline,tune,stemma,dividing_line,transmission_line,course,short_letter,crinkle,phone_line,bank_line,argumentation,business,wrinkle,telephone_line,blood,agate_line,pipeline,pedigree,descent,line_of_products,subscriber_line,rail_line,parentage,melodic_line,melodic_phrase</rdfs:comment>
        <rdfs:comment xml:lang="callstatement">LineDetectedCondition</rdfs:comment>
        <rdfs:comment xml:lang="importstatement">edu.kit.ipd.ev3.conditions.LineDetectedCondition</rdfs:comment>
        <rdfs:label xml:lang="en">ConditionLineDetected</rdfs:label>
    </owl:NamedIndividual>
    


    <!-- Optional[http://www.semanticweb.org/team3/robo-ontology-0]/#ConditionNearObject_2885ebd1_5cfe_415c_bef6_ed1585d260e0 -->

    <owl:NamedIndividual rdf:about="Optional[http://www.semanticweb.org/team3/robo-ontology-0]/#ConditionNearObject_2885ebd1_5cfe_415c_bef6_ed1585d260e0">
        <rdf:type rdf:resource="http://www.semanticweb.org/team3/robo-ontology-0#Method"/>
        <hasParameter rdf:resource="Optional[http://www.semanticweb.org/team3/robo-ontology-0]/#object_af319d4f_f219_4895_8cde_63607b4334c2"/>
        <rdfs:comment xml:lang="callstatement">IsNearObjectCondition</rdfs:comment>
        <rdfs:comment xml:lang="synonym">Near: cheeseparing,approximate,skinny,near,dear,close,penny-pinching,good,nigh</rdfs:comment>
        <rdfs:comment xml:lang="importstatement">edu.kit.ipd.ev3.conditions.IsNearObjectCondition</rdfs:comment>
        <rdfs:label xml:lang="en">ConditionNearObject</rdfs:label>
    </owl:NamedIndividual>
    


    <!-- Optional[http://www.semanticweb.org/team3/robo-ontology-0]/#ConditionSeesColor_cd5a4bb8_73ff_4856_8f34_4d344853faef -->

    <owl:NamedIndividual rdf:about="Optional[http://www.semanticweb.org/team3/robo-ontology-0]/#ConditionSeesColor_cd5a4bb8_73ff_4856_8f34_4d344853faef">
        <rdf:type rdf:resource="http://www.semanticweb.org/team3/robo-ontology-0#Method"/>
        <hasParameter rdf:resource="Optional[http://www.semanticweb.org/team3/robo-ontology-0]/#color_d1c9c023_a465_4b83_ae1b_bf6fddbafb96"/>
        <rdfs:comment xml:lang="synonym">Color: colouration,colour,vividness,semblance,color,gloss,coloration,coloring,colouring_material,colouring,coloring_material</rdfs:comment>
        <rdfs:comment xml:lang="synonym">Sees:</rdfs:comment>
        <rdfs:comment xml:lang="callstatement">SeesColorCondition</rdfs:comment>
        <rdfs:comment xml:lang="importstatement">edu.kit.ipd.ev3.conditions.SeesColorCondition</rdfs:comment>
        <rdfs:label xml:lang="en">ConditionSeesColor</rdfs:label>
    </owl:NamedIndividual>
    


    <!-- Optional[http://www.semanticweb.org/team3/robo-ontology-0]/#ConditionSeesObject_7e9019ee_89e0_4074_a791_7c746017f48a -->

    <owl:NamedIndividual rdf:about="Optional[http://www.semanticweb.org/team3/robo-ontology-0]/#ConditionSeesObject_7e9019ee_89e0_4074_a791_7c746017f48a">
        <rdf:type rdf:resource="http://www.semanticweb.org/team3/robo-ontology-0#Method"/>
        <hasParameter rdf:resource="Optional[http://www.semanticweb.org/team3/robo-ontology-0]/#object_b117c778_2f59_4e4e_b69b_f7dd8e3a4e21"/>
        <rdfs:comment xml:lang="synonym">Sees:</rdfs:comment>
        <rdfs:comment xml:lang="callstatement">SeesObjectCondition</rdfs:comment>
        <rdfs:comment xml:lang="importstatement">edu.kit.ipd.ev3.conditions.SeesObjectCondition</rdfs:comment>
        <rdfs:label xml:lang="en">ConditionSeesObject</rdfs:label>
    </owl:NamedIndividual>
    


    <!-- Optional[http://www.semanticweb.org/team3/robo-ontology-0]/#ConditionSeesRemote_e58532d7_fab9_464b_b33d_fe01e5ea353c -->

    <owl:NamedIndividual rdf:about="Optional[http://www.semanticweb.org/team3/robo-ontology-0]/#ConditionSeesRemote_e58532d7_fab9_464b_b33d_fe01e5ea353c">
        <rdf:type rdf:resource="http://www.semanticweb.org/team3/robo-ontology-0#Method"/>
        <rdfs:comment xml:lang="synonym">Remote: removed,outside,distant,remote,outback</rdfs:comment>
        <rdfs:comment xml:lang="synonym">Sees:</rdfs:comment>
        <rdfs:comment xml:lang="callstatement">SeesRemoteCondition</rdfs:comment>
        <rdfs:comment xml:lang="importstatement">edu.kit.ipd.ev3.conditions.SeesRemoteCondition</rdfs:comment>
        <rdfs:label xml:lang="en">ConditionSeesRemote</rdfs:label>
    </owl:NamedIndividual>
    


    <!-- Optional[http://www.semanticweb.org/team3/robo-ontology-0]/#Direction -->

    <owl:NamedIndividual rdf:about="Optional[http://www.semanticweb.org/team3/robo-ontology-0]/#Direction">
        <rdf:type rdf:resource="http://www.semanticweb.org/team3/robo-ontology-0#DataType"/>
        <hasValue rdf:resource="Optional[http://www.semanticweb.org/team3/robo-ontology-0]/#backward"/>
        <hasValue rdf:resource="Optional[http://www.semanticweb.org/team3/robo-ontology-0]/#down"/>
        <hasValue rdf:resource="Optional[http://www.semanticweb.org/team3/robo-ontology-0]/#forward"/>
        <hasValue rdf:resource="Optional[http://www.semanticweb.org/team3/robo-ontology-0]/#left"/>
        <hasValue rdf:resource="Optional[http://www.semanticweb.org/team3/robo-ontology-0]/#right"/>
        <hasValue rdf:resource="Optional[http://www.semanticweb.org/team3/robo-ontology-0]/#up"/>
        <rdfs:comment xml:lang="synonym">Direction: counsel,charge,counseling,focussing,steering,focus,focusing,focal_point,way,counselling,guidance,management,instruction,commission,centering,direction</rdfs:comment>
    </owl:NamedIndividual>
    


    <!-- Optional[http://www.semanticweb.org/team3/robo-ontology-0]/#ICondition -->

    <owl:NamedIndividual rdf:about="Optional[http://www.semanticweb.org/team3/robo-ontology-0]/#ICondition">
        <rdf:type rdf:resource="http://www.semanticweb.org/team3/robo-ontology-0#DataType"/>
        <rdfs:comment xml:lang="synonym">Condition: condition,shape,strings,circumstance,experimental_condition,consideration,term,precondition,stipulation,status</rdfs:comment>
    </owl:NamedIndividual>
    


    <!-- Optional[http://www.semanticweb.org/team3/robo-ontology-0]/#Revolution -->

    <owl:NamedIndividual rdf:about="Optional[http://www.semanticweb.org/team3/robo-ontology-0]/#Revolution">
        <rdf:type rdf:resource="http://www.semanticweb.org/team3/robo-ontology-0#DataType"/>
        <hasValue rdf:resource="Optional[http://www.semanticweb.org/team3/robo-ontology-0]/#full"/>
        <hasValue rdf:resource="Optional[http://www.semanticweb.org/team3/robo-ontology-0]/#half"/>
        <hasValue rdf:resource="Optional[http://www.semanticweb.org/team3/robo-ontology-0]/#quarter"/>
        <rdfs:comment xml:lang="synonym">Revolution: gyration,rotation,revolution</rdfs:comment>
    </owl:NamedIndividual>
    


    <!-- Optional[http://www.semanticweb.org/team3/robo-ontology-0]/#SceneryObject -->

    <owl:NamedIndividual rdf:about="Optional[http://www.semanticweb.org/team3/robo-ontology-0]/#SceneryObject">
        <rdf:type rdf:resource="http://www.semanticweb.org/team3/robo-ontology-0#DataType"/>
        <rdfs:comment xml:lang="synonym">Scenery: scenery,scene</rdfs:comment>
    </owl:NamedIndividual>
    


    <!-- Optional[http://www.semanticweb.org/team3/robo-ontology-0]/#Speed -->

    <owl:NamedIndividual rdf:about="Optional[http://www.semanticweb.org/team3/robo-ontology-0]/#Speed">
        <rdf:type rdf:resource="http://www.semanticweb.org/team3/robo-ontology-0#DataType"/>
        <rdf:type rdf:resource="http://www.semanticweb.org/team3/robo-ontology-0#Value"/>
        <hasValue rdf:resource="Optional[http://www.semanticweb.org/team3/robo-ontology-0]/#fast"/>
        <hasValue rdf:resource="Optional[http://www.semanticweb.org/team3/robo-ontology-0]/#fastest"/>
        <hasValue rdf:resource="Optional[http://www.semanticweb.org/team3/robo-ontology-0]/#medium"/>
        <hasValue rdf:resource="Optional[http://www.semanticweb.org/team3/robo-ontology-0]/#slow"/>
        <hasValue rdf:resource="Optional[http://www.semanticweb.org/team3/robo-ontology-0]/#slowest"/>
        <rdfs:comment xml:lang="synonym">Speed: focal_ratio,f_number,speeding,fastness,swiftness,upper,amphetamine,stop_number,pep_pill,velocity,hurrying,speed</rdfs:comment>
    </owl:NamedIndividual>
    


    <!-- Optional[http://www.semanticweb.org/team3/robo-ontology-0]/#backward -->

    <owl:NamedIndividual rdf:about="Optional[http://www.semanticweb.org/team3/robo-ontology-0]/#backward">
        <rdf:type rdf:resource="http://www.semanticweb.org/team3/robo-ontology-0#Value"/>
        <rdfs:comment xml:lang="callstatement">BACKWARD</rdfs:comment>
        <rdfs:comment xml:lang="synonym">backward: half-witted,feebleminded,backward,slow-witted</rdfs:comment>
        <rdfs:comment xml:lang="importstatement">edu.kit.ipd.ev3.enums.Direction</rdfs:comment>
    </owl:NamedIndividual>
    


    <!-- Optional[http://www.semanticweb.org/team3/robo-ontology-0]/#belch_28769a70_ee6a_47dd_b208_a1f25667fb98 -->

    <owl:NamedIndividual rdf:about="Optional[http://www.semanticweb.org/team3/robo-ontology-0]/#belch_28769a70_ee6a_47dd_b208_a1f25667fb98">
        <rdf:type rdf:resource="http://www.semanticweb.org/team3/robo-ontology-0#Method"/>
        <rdfs:comment xml:lang="callstatement">belch</rdfs:comment>
        <rdfs:comment xml:lang="synonym">belch: bubble,erupt,belch,eruct,extravasate,burp</rdfs:comment>
        <rdfs:comment xml:lang="importstatement">edu.kit.ipd.ev3.IRobo</rdfs:comment>
        <rdfs:label xml:lang="en">belch</rdfs:label>
    </owl:NamedIndividual>
    


    <!-- Optional[http://www.semanticweb.org/team3/robo-ontology-0]/#black -->

    <owl:NamedIndividual rdf:about="Optional[http://www.semanticweb.org/team3/robo-ontology-0]/#black">
        <rdf:type rdf:resource="http://www.semanticweb.org/team3/robo-ontology-0#Value"/>
        <rdfs:comment xml:lang="callstatement">BLACK</rdfs:comment>
        <rdfs:comment xml:lang="synonym">black: black-market,ignominious,smuggled,fateful,contraband,bootleg,calamitous,pitch-dark,black,disgraceful,opprobrious,dim,smutty,fatal,bleak,inglorious,disastrous,mordant,blackened,sinister,dark,shameful,pitch-black,grim</rdfs:comment>
        <rdfs:comment xml:lang="importstatement">edu.kit.ipd.ev3.enums.Color</rdfs:comment>
    </owl:NamedIndividual>
    


    <!-- Optional[http://www.semanticweb.org/team3/robo-ontology-0]/#blink_dba4b811_30ab_4865_b498_fc3c1c1c6c55 -->

    <owl:NamedIndividual rdf:about="Optional[http://www.semanticweb.org/team3/robo-ontology-0]/#blink_dba4b811_30ab_4865_b498_fc3c1c1c6c55">
        <rdf:type rdf:resource="http://www.semanticweb.org/team3/robo-ontology-0#Method"/>
        <rdfs:comment xml:lang="callstatement">blink</rdfs:comment>
        <rdfs:comment xml:lang="synonym">blink: twinkle,winkle,nictate,blink_away,nictitate,wink,blink,flash</rdfs:comment>
        <rdfs:comment xml:lang="importstatement">edu.kit.ipd.ev3.IRobo</rdfs:comment>
        <rdfs:label xml:lang="en">blink</rdfs:label>
    </owl:NamedIndividual>
    


    <!-- Optional[http://www.semanticweb.org/team3/robo-ontology-0]/#blue -->

    <owl:NamedIndividual rdf:about="Optional[http://www.semanticweb.org/team3/robo-ontology-0]/#blue">
        <rdf:type rdf:resource="http://www.semanticweb.org/team3/robo-ontology-0#Value"/>
        <rdfs:comment xml:lang="callstatement">BLUE</rdfs:comment>
        <rdfs:comment xml:lang="synonym">blue: drab,blue-blooded,dingy,down,bluish,racy,profane,dispirited,down_in_the_mouth,low,sorry,aristocratic,gloomy,depressed,dark,gentle,naughty,gamey,aristocratical,blasphemous,puritanical,puritanic,risque,low-spirited,dismal,blueish,spicy,dreary,downhearted,blue,disconsolate,gamy,downcast,juicy,patrician,drear,grim</rdfs:comment>
        <rdfs:comment xml:lang="importstatement">edu.kit.ipd.ev3.enums.Color</rdfs:comment>
    </owl:NamedIndividual>
    


    <!-- Optional[http://www.semanticweb.org/team3/robo-ontology-0]/#brown -->

    <owl:NamedIndividual rdf:about="Optional[http://www.semanticweb.org/team3/robo-ontology-0]/#brown">
        <rdf:type rdf:resource="http://www.semanticweb.org/team3/robo-ontology-0#Value"/>
        <rdfs:comment xml:lang="callstatement">BROWN</rdfs:comment>
        <rdfs:comment xml:lang="synonym">brown: chocolate-brown,browned,brown,brownish,dark-brown</rdfs:comment>
        <rdfs:comment xml:lang="importstatement">edu.kit.ipd.ev3.enums.Color</rdfs:comment>
    </owl:NamedIndividual>
    


    <!-- Optional[http://www.semanticweb.org/team3/robo-ontology-0]/#clap_1aa775d3_be0f_492e_88ab_d5bf99aaf8a1 -->

    <owl:NamedIndividual rdf:about="Optional[http://www.semanticweb.org/team3/robo-ontology-0]/#clap_1aa775d3_be0f_492e_88ab_d5bf99aaf8a1">
        <rdf:type rdf:resource="http://www.semanticweb.org/team3/robo-ontology-0#Method"/>
        <rdfs:comment xml:lang="callstatement">clap</rdfs:comment>
        <rdfs:comment xml:lang="synonym">clap: spat,clap,acclaim,applaud</rdfs:comment>
        <rdfs:comment xml:lang="importstatement">edu.kit.ipd.ev3.IRobo</rdfs:comment>
        <rdfs:label xml:lang="en">clap</rdfs:label>
    </owl:NamedIndividual>
    


    <!-- Optional[http://www.semanticweb.org/team3/robo-ontology-0]/#color_d1c9c023_a465_4b83_ae1b_bf6fddbafb96 -->

    <owl:NamedIndividual rdf:about="Optional[http://www.semanticweb.org/team3/robo-ontology-0]/#color_d1c9c023_a465_4b83_ae1b_bf6fddbafb96">
        <rdf:type rdf:resource="http://www.semanticweb.org/team3/robo-ontology-0#Parameter"/>
        <ofDataType rdf:resource="Optional[http://www.semanticweb.org/team3/robo-ontology-0]/#Color"/>
        <rdfs:comment xml:lang="pos">0</rdfs:comment>
        <rdfs:label xml:lang="en">color</rdfs:label>
    </owl:NamedIndividual>
    


    <!-- Optional[http://www.semanticweb.org/team3/robo-ontology-0]/#condition_1fa277eb_6ad6_4375_b1bf_a235bc5c60d0 -->

    <owl:NamedIndividual rdf:about="Optional[http://www.semanticweb.org/team3/robo-ontology-0]/#condition_1fa277eb_6ad6_4375_b1bf_a235bc5c60d0">
        <rdf:type rdf:resource="http://www.semanticweb.org/team3/robo-ontology-0#Parameter"/>
        <ofDataType rdf:resource="Optional[http://www.semanticweb.org/team3/robo-ontology-0]/#ICondition"/>
        <rdfs:comment xml:lang="pos">1</rdfs:comment>
        <rdfs:label xml:lang="en">condition</rdfs:label>
    </owl:NamedIndividual>
    


    <!-- Optional[http://www.semanticweb.org/team3/robo-ontology-0]/#condition_236a119c_ede1_43c8_968f_9ce1f5d0fa43 -->

    <owl:NamedIndividual rdf:about="Optional[http://www.semanticweb.org/team3/robo-ontology-0]/#condition_236a119c_ede1_43c8_968f_9ce1f5d0fa43">
        <rdf:type rdf:resource="http://www.semanticweb.org/team3/robo-ontology-0#Parameter"/>
        <ofDataType rdf:resource="Optional[http://www.semanticweb.org/team3/robo-ontology-0]/#ICondition"/>
        <rdfs:comment xml:lang="pos">0</rdfs:comment>
        <rdfs:label xml:lang="en">condition</rdfs:label>
    </owl:NamedIndividual>
    


    <!-- Optional[http://www.semanticweb.org/team3/robo-ontology-0]/#condition_687e8b9b_70ee_48e1_9c10_20690d138d25 -->

    <owl:NamedIndividual rdf:about="Optional[http://www.semanticweb.org/team3/robo-ontology-0]/#condition_687e8b9b_70ee_48e1_9c10_20690d138d25">
        <rdf:type rdf:resource="http://www.semanticweb.org/team3/robo-ontology-0#Parameter"/>
        <ofDataType rdf:resource="Optional[http://www.semanticweb.org/team3/robo-ontology-0]/#ICondition"/>
        <rdfs:comment xml:lang="pos">1</rdfs:comment>
        <rdfs:label xml:lang="en">condition</rdfs:label>
    </owl:NamedIndividual>
    


    <!-- Optional[http://www.semanticweb.org/team3/robo-ontology-0]/#condition_a3c803d5_599a_43e5_b84c_804641653f37 -->

    <owl:NamedIndividual rdf:about="Optional[http://www.semanticweb.org/team3/robo-ontology-0]/#condition_a3c803d5_599a_43e5_b84c_804641653f37">
        <rdf:type rdf:resource="http://www.semanticweb.org/team3/robo-ontology-0#Parameter"/>
        <ofDataType rdf:resource="Optional[http://www.semanticweb.org/team3/robo-ontology-0]/#ICondition"/>
        <rdfs:comment xml:lang="pos">0</rdfs:comment>
        <rdfs:label xml:lang="en">condition</rdfs:label>
    </owl:NamedIndividual>
    


    <!-- Optional[http://www.semanticweb.org/team3/robo-ontology-0]/#condition_ac983e93_487b_498b_9ea0_c1f1009739fd -->

    <owl:NamedIndividual rdf:about="Optional[http://www.semanticweb.org/team3/robo-ontology-0]/#condition_ac983e93_487b_498b_9ea0_c1f1009739fd">
        <rdf:type rdf:resource="http://www.semanticweb.org/team3/robo-ontology-0#Parameter"/>
        <ofDataType rdf:resource="Optional[http://www.semanticweb.org/team3/robo-ontology-0]/#ICondition"/>
        <rdfs:comment xml:lang="pos">1</rdfs:comment>
        <rdfs:label xml:lang="en">condition</rdfs:label>
    </owl:NamedIndividual>
    


    <!-- Optional[http://www.semanticweb.org/team3/robo-ontology-0]/#condition_c26dbe68_f60f_4635_b13f_e238d4432256 -->

    <owl:NamedIndividual rdf:about="Optional[http://www.semanticweb.org/team3/robo-ontology-0]/#condition_c26dbe68_f60f_4635_b13f_e238d4432256">
        <rdf:type rdf:resource="http://www.semanticweb.org/team3/robo-ontology-0#Parameter"/>
        <ofDataType rdf:resource="Optional[http://www.semanticweb.org/team3/robo-ontology-0]/#ICondition"/>
        <rdfs:comment xml:lang="pos">2</rdfs:comment>
        <rdfs:label xml:lang="en">condition</rdfs:label>
    </owl:NamedIndividual>
    


    <!-- Optional[http://www.semanticweb.org/team3/robo-ontology-0]/#condition_c9954084_3136_4c88_a6e5_13b0496b2642 -->

    <owl:NamedIndividual rdf:about="Optional[http://www.semanticweb.org/team3/robo-ontology-0]/#condition_c9954084_3136_4c88_a6e5_13b0496b2642">
        <rdf:type rdf:resource="http://www.semanticweb.org/team3/robo-ontology-0#Parameter"/>
        <ofDataType rdf:resource="Optional[http://www.semanticweb.org/team3/robo-ontology-0]/#ICondition"/>
        <rdfs:comment xml:lang="pos">1</rdfs:comment>
        <rdfs:label xml:lang="en">condition</rdfs:label>
    </owl:NamedIndividual>
    


    <!-- Optional[http://www.semanticweb.org/team3/robo-ontology-0]/#condition_f2c54d55_fac2_4c1f_a8c9_f7e225fd2f9a -->

    <owl:NamedIndividual rdf:about="Optional[http://www.semanticweb.org/team3/robo-ontology-0]/#condition_f2c54d55_fac2_4c1f_a8c9_f7e225fd2f9a">
        <rdf:type rdf:resource="http://www.semanticweb.org/team3/robo-ontology-0#Parameter"/>
        <ofDataType rdf:resource="Optional[http://www.semanticweb.org/team3/robo-ontology-0]/#ICondition"/>
        <rdfs:comment xml:lang="pos">0</rdfs:comment>
        <rdfs:label xml:lang="en">condition</rdfs:label>
    </owl:NamedIndividual>
    


    <!-- Optional[http://www.semanticweb.org/team3/robo-ontology-0]/#degrees_1d01bf9a_b37b_4e6b_9269_02a14a71a377 -->

    <owl:NamedIndividual rdf:about="Optional[http://www.semanticweb.org/team3/robo-ontology-0]/#degrees_1d01bf9a_b37b_4e6b_9269_02a14a71a377">
        <rdf:type rdf:resource="http://www.semanticweb.org/team3/robo-ontology-0#Parameter"/>
        <ofDataType rdf:resource="Optional[http://www.semanticweb.org/team3/robo-ontology-0]/#int"/>
        <rdfs:comment xml:lang="pos">1</rdfs:comment>
        <rdfs:label xml:lang="en">degrees</rdfs:label>
    </owl:NamedIndividual>
    


    <!-- Optional[http://www.semanticweb.org/team3/robo-ontology-0]/#degrees_86efca15_f77e_4e27_8f39_667885e65e6b -->

    <owl:NamedIndividual rdf:about="Optional[http://www.semanticweb.org/team3/robo-ontology-0]/#degrees_86efca15_f77e_4e27_8f39_667885e65e6b">
        <rdf:type rdf:resource="http://www.semanticweb.org/team3/robo-ontology-0#Parameter"/>
        <ofDataType rdf:resource="Optional[http://www.semanticweb.org/team3/robo-ontology-0]/#int"/>
        <rdfs:comment xml:lang="pos">0</rdfs:comment>
        <rdfs:label xml:lang="en">degrees</rdfs:label>
    </owl:NamedIndividual>
    


    <!-- Optional[http://www.semanticweb.org/team3/robo-ontology-0]/#degrees_97cd9f0f_1f53_4edd_b95e_f3888dfdcc25 -->

    <owl:NamedIndividual rdf:about="Optional[http://www.semanticweb.org/team3/robo-ontology-0]/#degrees_97cd9f0f_1f53_4edd_b95e_f3888dfdcc25">
        <rdf:type rdf:resource="http://www.semanticweb.org/team3/robo-ontology-0#Parameter"/>
        <ofDataType rdf:resource="Optional[http://www.semanticweb.org/team3/robo-ontology-0]/#int"/>
        <rdfs:comment xml:lang="pos">1</rdfs:comment>
        <rdfs:label xml:lang="en">degrees</rdfs:label>
    </owl:NamedIndividual>
    


    <!-- Optional[http://www.semanticweb.org/team3/robo-ontology-0]/#degrees_bcac42d9_845b_48b8_bb49_703c21041c26 -->

    <owl:NamedIndividual rdf:about="Optional[http://www.semanticweb.org/team3/robo-ontology-0]/#degrees_bcac42d9_845b_48b8_bb49_703c21041c26">
        <rdf:type rdf:resource="http://www.semanticweb.org/team3/robo-ontology-0#Parameter"/>
        <ofDataType rdf:resource="Optional[http://www.semanticweb.org/team3/robo-ontology-0]/#int"/>
        <rdfs:comment xml:lang="pos">0</rdfs:comment>
        <rdfs:label xml:lang="en">degrees</rdfs:label>
    </owl:NamedIndividual>
    


    <!-- Optional[http://www.semanticweb.org/team3/robo-ontology-0]/#dir_105a0f66_e5d0_47dd_b6b4_e88b4dcaf3a5 -->

    <owl:NamedIndividual rdf:about="Optional[http://www.semanticweb.org/team3/robo-ontology-0]/#dir_105a0f66_e5d0_47dd_b6b4_e88b4dcaf3a5">
        <rdf:type rdf:resource="http://www.semanticweb.org/team3/robo-ontology-0#Parameter"/>
        <ofDataType rdf:resource="Optional[http://www.semanticweb.org/team3/robo-ontology-0]/#Direction"/>
        <rdfs:comment xml:lang="pos">0</rdfs:comment>
        <rdfs:label xml:lang="en">dir</rdfs:label>
    </owl:NamedIndividual>
    


    <!-- Optional[http://www.semanticweb.org/team3/robo-ontology-0]/#dir_17ceb3d5_f0c6_4c6c_bf2c_55af1027d5b3 -->

    <owl:NamedIndividual rdf:about="Optional[http://www.semanticweb.org/team3/robo-ontology-0]/#dir_17ceb3d5_f0c6_4c6c_bf2c_55af1027d5b3">
        <rdf:type rdf:resource="http://www.semanticweb.org/team3/robo-ontology-0#Parameter"/>
        <ofDataType rdf:resource="Optional[http://www.semanticweb.org/team3/robo-ontology-0]/#Direction"/>
        <rdfs:comment xml:lang="pos">0</rdfs:comment>
        <rdfs:label xml:lang="en">dir</rdfs:label>
    </owl:NamedIndividual>
    


    <!-- Optional[http://www.semanticweb.org/team3/robo-ontology-0]/#dir_2650cea4_8219_42ad_8c2d_32aa10504a2e -->

    <owl:NamedIndividual rdf:about="Optional[http://www.semanticweb.org/team3/robo-ontology-0]/#dir_2650cea4_8219_42ad_8c2d_32aa10504a2e">
        <rdf:type rdf:resource="http://www.semanticweb.org/team3/robo-ontology-0#Parameter"/>
        <ofDataType rdf:resource="Optional[http://www.semanticweb.org/team3/robo-ontology-0]/#Direction"/>
        <rdfs:comment xml:lang="pos">0</rdfs:comment>
        <rdfs:label xml:lang="en">dir</rdfs:label>
    </owl:NamedIndividual>
    


    <!-- Optional[http://www.semanticweb.org/team3/robo-ontology-0]/#dir_2882212f_ba3e_4547_a62c_fcf356ce5ca3 -->

    <owl:NamedIndividual rdf:about="Optional[http://www.semanticweb.org/team3/robo-ontology-0]/#dir_2882212f_ba3e_4547_a62c_fcf356ce5ca3">
        <rdf:type rdf:resource="http://www.semanticweb.org/team3/robo-ontology-0#Parameter"/>
        <ofDataType rdf:resource="Optional[http://www.semanticweb.org/team3/robo-ontology-0]/#Direction"/>
        <rdfs:comment xml:lang="pos">0</rdfs:comment>
        <rdfs:label xml:lang="en">dir</rdfs:label>
    </owl:NamedIndividual>
    


    <!-- Optional[http://www.semanticweb.org/team3/robo-ontology-0]/#dir_3e10eb90_4969_4f3a_a5ef_d45c1f342e86 -->

    <owl:NamedIndividual rdf:about="Optional[http://www.semanticweb.org/team3/robo-ontology-0]/#dir_3e10eb90_4969_4f3a_a5ef_d45c1f342e86">
        <rdf:type rdf:resource="http://www.semanticweb.org/team3/robo-ontology-0#Parameter"/>
        <ofDataType rdf:resource="Optional[http://www.semanticweb.org/team3/robo-ontology-0]/#Direction"/>
        <rdfs:comment xml:lang="pos">0</rdfs:comment>
        <rdfs:label xml:lang="en">dir</rdfs:label>
    </owl:NamedIndividual>
    


    <!-- Optional[http://www.semanticweb.org/team3/robo-ontology-0]/#dir_456efe65_c422_4fd1_804d_82a2f74ef433 -->

    <owl:NamedIndividual rdf:about="Optional[http://www.semanticweb.org/team3/robo-ontology-0]/#dir_456efe65_c422_4fd1_804d_82a2f74ef433">
        <rdf:type rdf:resource="http://www.semanticweb.org/team3/robo-ontology-0#Parameter"/>
        <ofDataType rdf:resource="Optional[http://www.semanticweb.org/team3/robo-ontology-0]/#Direction"/>
        <rdfs:comment xml:lang="pos">0</rdfs:comment>
        <rdfs:label xml:lang="en">dir</rdfs:label>
    </owl:NamedIndividual>
    


    <!-- Optional[http://www.semanticweb.org/team3/robo-ontology-0]/#dir_4d27670d_4910_4c3e_99f7_c6b76468ebbd -->

    <owl:NamedIndividual rdf:about="Optional[http://www.semanticweb.org/team3/robo-ontology-0]/#dir_4d27670d_4910_4c3e_99f7_c6b76468ebbd">
        <rdf:type rdf:resource="http://www.semanticweb.org/team3/robo-ontology-0#Parameter"/>
        <ofDataType rdf:resource="Optional[http://www.semanticweb.org/team3/robo-ontology-0]/#Direction"/>
        <rdfs:comment xml:lang="pos">0</rdfs:comment>
        <rdfs:label xml:lang="en">dir</rdfs:label>
    </owl:NamedIndividual>
    


    <!-- Optional[http://www.semanticweb.org/team3/robo-ontology-0]/#dir_5ec1806c_1162_4df5_b998_7d0f64c07c18 -->

    <owl:NamedIndividual rdf:about="Optional[http://www.semanticweb.org/team3/robo-ontology-0]/#dir_5ec1806c_1162_4df5_b998_7d0f64c07c18">
        <rdf:type rdf:resource="http://www.semanticweb.org/team3/robo-ontology-0#Parameter"/>
        <ofDataType rdf:resource="Optional[http://www.semanticweb.org/team3/robo-ontology-0]/#Direction"/>
        <rdfs:comment xml:lang="pos">0</rdfs:comment>
        <rdfs:label xml:lang="en">dir</rdfs:label>
    </owl:NamedIndividual>
    


    <!-- Optional[http://www.semanticweb.org/team3/robo-ontology-0]/#dir_6c6821d0_0b6f_4abd_84a8_51d5562bebdd -->

    <owl:NamedIndividual rdf:about="Optional[http://www.semanticweb.org/team3/robo-ontology-0]/#dir_6c6821d0_0b6f_4abd_84a8_51d5562bebdd">
        <rdf:type rdf:resource="http://www.semanticweb.org/team3/robo-ontology-0#Parameter"/>
        <ofDataType rdf:resource="Optional[http://www.semanticweb.org/team3/robo-ontology-0]/#Direction"/>
        <rdfs:comment xml:lang="pos">0</rdfs:comment>
        <rdfs:label xml:lang="en">dir</rdfs:label>
    </owl:NamedIndividual>
    


    <!-- Optional[http://www.semanticweb.org/team3/robo-ontology-0]/#dir_7730cef1_1bed_43f3_8217_ab397f9f5aaa -->

    <owl:NamedIndividual rdf:about="Optional[http://www.semanticweb.org/team3/robo-ontology-0]/#dir_7730cef1_1bed_43f3_8217_ab397f9f5aaa">
        <rdf:type rdf:resource="http://www.semanticweb.org/team3/robo-ontology-0#Parameter"/>
        <ofDataType rdf:resource="Optional[http://www.semanticweb.org/team3/robo-ontology-0]/#Direction"/>
        <rdfs:comment xml:lang="pos">0</rdfs:comment>
        <rdfs:label xml:lang="en">dir</rdfs:label>
    </owl:NamedIndividual>
    


    <!-- Optional[http://www.semanticweb.org/team3/robo-ontology-0]/#dir_9a14702b_2d5e_4650_a755_934ab436b793 -->

    <owl:NamedIndividual rdf:about="Optional[http://www.semanticweb.org/team3/robo-ontology-0]/#dir_9a14702b_2d5e_4650_a755_934ab436b793">
        <rdf:type rdf:resource="http://www.semanticweb.org/team3/robo-ontology-0#Parameter"/>
        <ofDataType rdf:resource="Optional[http://www.semanticweb.org/team3/robo-ontology-0]/#Direction"/>
        <rdfs:comment xml:lang="pos">0</rdfs:comment>
        <rdfs:label xml:lang="en">dir</rdfs:label>
    </owl:NamedIndividual>
    


    <!-- Optional[http://www.semanticweb.org/team3/robo-ontology-0]/#dir_9b678577_ca1c_4506_bdd2_82f9c0e20595 -->

    <owl:NamedIndividual rdf:about="Optional[http://www.semanticweb.org/team3/robo-ontology-0]/#dir_9b678577_ca1c_4506_bdd2_82f9c0e20595">
        <rdf:type rdf:resource="http://www.semanticweb.org/team3/robo-ontology-0#Parameter"/>
        <ofDataType rdf:resource="Optional[http://www.semanticweb.org/team3/robo-ontology-0]/#Direction"/>
        <rdfs:comment xml:lang="pos">0</rdfs:comment>
        <rdfs:label xml:lang="en">dir</rdfs:label>
    </owl:NamedIndividual>
    


    <!-- Optional[http://www.semanticweb.org/team3/robo-ontology-0]/#dir_abb1381b_479c_4ce3_a599_6cb3441ebf89 -->

    <owl:NamedIndividual rdf:about="Optional[http://www.semanticweb.org/team3/robo-ontology-0]/#dir_abb1381b_479c_4ce3_a599_6cb3441ebf89">
        <rdf:type rdf:resource="http://www.semanticweb.org/team3/robo-ontology-0#Parameter"/>
        <ofDataType rdf:resource="Optional[http://www.semanticweb.org/team3/robo-ontology-0]/#Direction"/>
        <rdfs:comment xml:lang="pos">0</rdfs:comment>
        <rdfs:label xml:lang="en">dir</rdfs:label>
    </owl:NamedIndividual>
    


    <!-- Optional[http://www.semanticweb.org/team3/robo-ontology-0]/#dir_c2408af1_cd85_4bce_bf9a_93015ed8bf5e -->

    <owl:NamedIndividual rdf:about="Optional[http://www.semanticweb.org/team3/robo-ontology-0]/#dir_c2408af1_cd85_4bce_bf9a_93015ed8bf5e">
        <rdf:type rdf:resource="http://www.semanticweb.org/team3/robo-ontology-0#Parameter"/>
        <ofDataType rdf:resource="Optional[http://www.semanticweb.org/team3/robo-ontology-0]/#Direction"/>
        <rdfs:comment xml:lang="pos">0</rdfs:comment>
        <rdfs:label xml:lang="en">dir</rdfs:label>
    </owl:NamedIndividual>
    


    <!-- Optional[http://www.semanticweb.org/team3/robo-ontology-0]/#dir_d2165658_484a_4759_89b6_a53ec9c2e631 -->

    <owl:NamedIndividual rdf:about="Optional[http://www.semanticweb.org/team3/robo-ontology-0]/#dir_d2165658_484a_4759_89b6_a53ec9c2e631">
        <rdf:type rdf:resource="http://www.semanticweb.org/team3/robo-ontology-0#Parameter"/>
        <ofDataType rdf:resource="Optional[http://www.semanticweb.org/team3/robo-ontology-0]/#Direction"/>
        <rdfs:comment xml:lang="pos">0</rdfs:comment>
        <rdfs:label xml:lang="en">dir</rdfs:label>
    </owl:NamedIndividual>
    


    <!-- Optional[http://www.semanticweb.org/team3/robo-ontology-0]/#direction_30496b80_b00f_4f70_809f_fdd7032448e8 -->

    <owl:NamedIndividual rdf:about="Optional[http://www.semanticweb.org/team3/robo-ontology-0]/#direction_30496b80_b00f_4f70_809f_fdd7032448e8">
        <rdf:type rdf:resource="http://www.semanticweb.org/team3/robo-ontology-0#Parameter"/>
        <ofDataType rdf:resource="Optional[http://www.semanticweb.org/team3/robo-ontology-0]/#Direction"/>
        <rdfs:comment xml:lang="pos">0</rdfs:comment>
        <rdfs:label xml:lang="en">direction</rdfs:label>
    </owl:NamedIndividual>
    


    <!-- Optional[http://www.semanticweb.org/team3/robo-ontology-0]/#direction_c6aeeb65_4287_41e0_8fec_371521e2d3e7 -->

    <owl:NamedIndividual rdf:about="Optional[http://www.semanticweb.org/team3/robo-ontology-0]/#direction_c6aeeb65_4287_41e0_8fec_371521e2d3e7">
        <rdf:type rdf:resource="http://www.semanticweb.org/team3/robo-ontology-0#Parameter"/>
        <ofDataType rdf:resource="Optional[http://www.semanticweb.org/team3/robo-ontology-0]/#Direction"/>
        <rdfs:comment xml:lang="pos">0</rdfs:comment>
        <rdfs:label xml:lang="en">direction</rdfs:label>
    </owl:NamedIndividual>
    


    <!-- Optional[http://www.semanticweb.org/team3/robo-ontology-0]/#down -->

    <owl:NamedIndividual rdf:about="Optional[http://www.semanticweb.org/team3/robo-ontology-0]/#down">
        <rdf:type rdf:resource="http://www.semanticweb.org/team3/robo-ontology-0#Value"/>
        <rdfs:comment xml:lang="callstatement">DOWN</rdfs:comment>
        <rdfs:comment xml:lang="synonym">down: downward,low-spirited,down,mastered,downhearted,down_pat,dispirited,blue,down_in_the_mouth,low,downcast,depressed,gloomy,grim</rdfs:comment>
        <rdfs:comment xml:lang="importstatement">edu.kit.ipd.ev3.enums.Direction</rdfs:comment>
    </owl:NamedIndividual>
    


    <!-- Optional[http://www.semanticweb.org/team3/robo-ontology-0]/#fast -->

    <owl:NamedIndividual rdf:about="Optional[http://www.semanticweb.org/team3/robo-ontology-0]/#fast">
        <rdf:type rdf:resource="http://www.semanticweb.org/team3/robo-ontology-0#Value"/>
        <rdfs:comment xml:lang="callstatement">FAST</rdfs:comment>
        <rdfs:comment xml:lang="importstatement">edu.kit.ipd.ev3.enums.Speed</rdfs:comment>
        <rdfs:comment xml:lang="synonym">fast: quick,debauched,dissipated,loyal,dissolute,immobile,degraded,libertine,degenerate,firm,fast,riotous,flying,truehearted,profligate</rdfs:comment>
    </owl:NamedIndividual>
    


    <!-- Optional[http://www.semanticweb.org/team3/robo-ontology-0]/#fastest -->

    <owl:NamedIndividual rdf:about="Optional[http://www.semanticweb.org/team3/robo-ontology-0]/#fastest">
        <rdf:type rdf:resource="http://www.semanticweb.org/team3/robo-ontology-0#Value"/>
        <rdfs:comment xml:lang="callstatement">FASTEST</rdfs:comment>
        <rdfs:comment xml:lang="importstatement">edu.kit.ipd.ev3.enums.Speed</rdfs:comment>
        <rdfs:comment xml:lang="synonym">fastest:</rdfs:comment>
    </owl:NamedIndividual>
    


    <!-- Optional[http://www.semanticweb.org/team3/robo-ontology-0]/#followLineUntil_47c773f2_f939_41b7_a770_2f4a90b49e2e -->

    <owl:NamedIndividual rdf:about="Optional[http://www.semanticweb.org/team3/robo-ontology-0]/#followLineUntil_47c773f2_f939_41b7_a770_2f4a90b49e2e">
        <rdf:type rdf:resource="http://www.semanticweb.org/team3/robo-ontology-0#Method"/>
        <hasParameter rdf:resource="Optional[http://www.semanticweb.org/team3/robo-ontology-0]/#condition_687e8b9b_70ee_48e1_9c10_20690d138d25"/>
        <hasParameter rdf:resource="Optional[http://www.semanticweb.org/team3/robo-ontology-0]/#speed_e1d0e420_4dfb_4fe4_b44b_4a3644e6d36c"/>
        <rdfs:comment xml:lang="synonym">Line: lineage,argument,occupation,channel,personal_credit_line,production_line,line_of_credit,logical_argument,credit_line,business_line,stock,cable,blood_line,line_of_work,strain,demarcation,telephone_circuit,assembly_line,line_of_merchandise,product_line,melody,line_of_business,personal_line_of_credit,contrast,crease,line_of_descent,job,communication_channel,note,furrow,ancestry,billet,line_of_reasoning,line,railway_line,origin,seam,air,bloodline,tune,stemma,dividing_line,transmission_line,course,short_letter,crinkle,phone_line,bank_line,argumentation,business,wrinkle,telephone_line,blood,agate_line,pipeline,pedigree,descent,line_of_products,subscriber_line,rail_line,parentage,melodic_line,melodic_phrase</rdfs:comment>
        <rdfs:comment xml:lang="importstatement">edu.kit.ipd.ev3.IRobo</rdfs:comment>
        <rdfs:comment xml:lang="synonym">follow: keep_up,be,stick_to,come_after,espouse,watch_over,observe,trace,pursue,fall_out,keep_abreast,play_along,keep_an_eye_on,comply,conform_to,postdate,come,travel_along,follow,take_after,accompany,surveil,watch,adopt,succeed,stick_with,survey,abide_by</rdfs:comment>
        <rdfs:comment xml:lang="callstatement">followLineUntil</rdfs:comment>
        <rdfs:label xml:lang="en">followLineUntil</rdfs:label>
    </owl:NamedIndividual>
    


    <!-- Optional[http://www.semanticweb.org/team3/robo-ontology-0]/#followLineUntil_b1141948_f721_4f2f_ab17_db74fbc5fb10 -->

    <owl:NamedIndividual rdf:about="Optional[http://www.semanticweb.org/team3/robo-ontology-0]/#followLineUntil_b1141948_f721_4f2f_ab17_db74fbc5fb10">
        <rdf:type rdf:resource="http://www.semanticweb.org/team3/robo-ontology-0#Method"/>
        <hasParameter rdf:resource="Optional[http://www.semanticweb.org/team3/robo-ontology-0]/#condition_a3c803d5_599a_43e5_b84c_804641653f37"/>
        <rdfs:comment xml:lang="synonym">Line: lineage,argument,occupation,channel,personal_credit_line,production_line,line_of_credit,logical_argument,credit_line,business_line,stock,cable,blood_line,line_of_work,strain,demarcation,telephone_circuit,assembly_line,line_of_merchandise,product_line,melody,line_of_business,personal_line_of_credit,contrast,crease,line_of_descent,job,communication_channel,note,furrow,ancestry,billet,line_of_reasoning,line,railway_line,origin,seam,air,bloodline,tune,stemma,dividing_line,transmission_line,course,short_letter,crinkle,phone_line,bank_line,argumentation,business,wrinkle,telephone_line,blood,agate_line,pipeline,pedigree,descent,line_of_products,subscriber_line,rail_line,parentage,melodic_line,melodic_phrase</rdfs:comment>
        <rdfs:comment xml:lang="importstatement">edu.kit.ipd.ev3.IRobo</rdfs:comment>
        <rdfs:comment xml:lang="synonym">follow: keep_up,be,stick_to,come_after,espouse,watch_over,observe,trace,pursue,fall_out,keep_abreast,play_along,keep_an_eye_on,comply,conform_to,postdate,come,travel_along,follow,take_after,accompany,surveil,watch,adopt,succeed,stick_with,survey,abide_by</rdfs:comment>
        <rdfs:comment xml:lang="callstatement">followLineUntil</rdfs:comment>
        <rdfs:label xml:lang="en">followLineUntil</rdfs:label>
    </owl:NamedIndividual>
    


    <!-- Optional[http://www.semanticweb.org/team3/robo-ontology-0]/#forward -->

    <owl:NamedIndividual rdf:about="Optional[http://www.semanticweb.org/team3/robo-ontology-0]/#forward">
        <rdf:type rdf:resource="http://www.semanticweb.org/team3/robo-ontology-0#Value"/>
        <rdfs:comment xml:lang="callstatement">FORWARD</rdfs:comment>
        <rdfs:comment xml:lang="importstatement">edu.kit.ipd.ev3.enums.Direction</rdfs:comment>
        <rdfs:comment xml:lang="synonym">forward: forward-moving,forward,advancing</rdfs:comment>
    </owl:NamedIndividual>
    


    <!-- Optional[http://www.semanticweb.org/team3/robo-ontology-0]/#full -->

    <owl:NamedIndividual rdf:about="Optional[http://www.semanticweb.org/team3/robo-ontology-0]/#full">
        <rdf:type rdf:resource="http://www.semanticweb.org/team3/robo-ontology-0#Value"/>
        <rdfs:comment xml:lang="callstatement">FULL</rdfs:comment>
        <rdfs:comment xml:lang="importstatement">edu.kit.ipd.ev3.enums.Revolution</rdfs:comment>
        <rdfs:comment xml:lang="synonym">full: total,wide,broad,replete,entire,wide-cut,good,full</rdfs:comment>
    </owl:NamedIndividual>
    


    <!-- Optional[http://www.semanticweb.org/team3/robo-ontology-0]/#grab_1d868109_1049_4bad_b334_f9289541520b -->

    <owl:NamedIndividual rdf:about="Optional[http://www.semanticweb.org/team3/robo-ontology-0]/#grab_1d868109_1049_4bad_b334_f9289541520b">
        <rdf:type rdf:resource="http://www.semanticweb.org/team3/robo-ontology-0#Method"/>
        <hasParameter rdf:resource="Optional[http://www.semanticweb.org/team3/robo-ontology-0]/#object_52a6de59_263a_4cfb_aa28_c86b12869ee7"/>
        <rdfs:comment xml:lang="importstatement">edu.kit.ipd.ev3.IRobo</rdfs:comment>
        <rdfs:comment xml:lang="callstatement">grab</rdfs:comment>
        <rdfs:comment xml:lang="synonym">grab: take_hold_of,seize,snaffle,catch,grab,snap_up</rdfs:comment>
        <rdfs:label xml:lang="en">grab</rdfs:label>
    </owl:NamedIndividual>
    


    <!-- Optional[http://www.semanticweb.org/team3/robo-ontology-0]/#green -->

    <owl:NamedIndividual rdf:about="Optional[http://www.semanticweb.org/team3/robo-ontology-0]/#green">
        <rdf:type rdf:resource="http://www.semanticweb.org/team3/robo-ontology-0#Value"/>
        <rdfs:comment xml:lang="callstatement">GREEN</rdfs:comment>
        <rdfs:comment xml:lang="importstatement">edu.kit.ipd.ev3.enums.Color</rdfs:comment>
        <rdfs:comment xml:lang="synonym">green: greenish,gullible,green,dark-green,light-green,fleeceable,immature,unripened,unripe</rdfs:comment>
    </owl:NamedIndividual>
    


    <!-- Optional[http://www.semanticweb.org/team3/robo-ontology-0]/#half -->

    <owl:NamedIndividual rdf:about="Optional[http://www.semanticweb.org/team3/robo-ontology-0]/#half">
        <rdf:type rdf:resource="http://www.semanticweb.org/team3/robo-ontology-0#Value"/>
        <rdfs:comment xml:lang="callstatement">HALF</rdfs:comment>
        <rdfs:comment xml:lang="importstatement">edu.kit.ipd.ev3.enums.Revolution</rdfs:comment>
        <rdfs:comment xml:lang="synonym">half: half</rdfs:comment>
    </owl:NamedIndividual>
    


    <!-- Optional[http://www.semanticweb.org/team3/robo-ontology-0]/#int -->

    <owl:NamedIndividual rdf:about="Optional[http://www.semanticweb.org/team3/robo-ontology-0]/#int">
        <rdf:type rdf:resource="http://www.semanticweb.org/team3/robo-ontology-0#DataType"/>
        <rdfs:comment xml:lang="synonym">int:</rdfs:comment>
    </owl:NamedIndividual>
    


    <!-- Optional[http://www.semanticweb.org/team3/robo-ontology-0]/#left -->

    <owl:NamedIndividual rdf:about="Optional[http://www.semanticweb.org/team3/robo-ontology-0]/#left">
        <rdf:type rdf:resource="http://www.semanticweb.org/team3/robo-ontology-0#Value"/>
        <rdfs:comment xml:lang="callstatement">LEFT</rdfs:comment>
        <rdfs:comment xml:lang="importstatement">edu.kit.ipd.ev3.enums.Direction</rdfs:comment>
        <rdfs:comment xml:lang="synonym">left: leftover,left,unexpended,left-hand,left_over,odd,remaining</rdfs:comment>
    </owl:NamedIndividual>
    


    <!-- Optional[http://www.semanticweb.org/team3/robo-ontology-0]/#length_1aae939b_0bc1_4a19_be30_1ab2a44dc159 -->

    <owl:NamedIndividual rdf:about="Optional[http://www.semanticweb.org/team3/robo-ontology-0]/#length_1aae939b_0bc1_4a19_be30_1ab2a44dc159">
        <rdf:type rdf:resource="http://www.semanticweb.org/team3/robo-ontology-0#Parameter"/>
        <ofDataType rdf:resource="Optional[http://www.semanticweb.org/team3/robo-ontology-0]/#int"/>
        <rdfs:comment xml:lang="pos">1</rdfs:comment>
        <rdfs:label xml:lang="en">length</rdfs:label>
    </owl:NamedIndividual>
    


    <!-- Optional[http://www.semanticweb.org/team3/robo-ontology-0]/#length_aa148b58_7162_4931_a0cf_af3a607ff503 -->

    <owl:NamedIndividual rdf:about="Optional[http://www.semanticweb.org/team3/robo-ontology-0]/#length_aa148b58_7162_4931_a0cf_af3a607ff503">
        <rdf:type rdf:resource="http://www.semanticweb.org/team3/robo-ontology-0#Parameter"/>
        <ofDataType rdf:resource="Optional[http://www.semanticweb.org/team3/robo-ontology-0]/#int"/>
        <rdfs:comment xml:lang="pos">1</rdfs:comment>
        <rdfs:label xml:lang="en">length</rdfs:label>
    </owl:NamedIndividual>
    


    <!-- Optional[http://www.semanticweb.org/team3/robo-ontology-0]/#liftHead_b56fe84f_82c1_4441_aecb_7c8624cff340 -->

    <owl:NamedIndividual rdf:about="Optional[http://www.semanticweb.org/team3/robo-ontology-0]/#liftHead_b56fe84f_82c1_4441_aecb_7c8624cff340">
        <rdf:type rdf:resource="http://www.semanticweb.org/team3/robo-ontology-0#Method"/>
        <rdfs:comment xml:lang="synonym">Head: top_dog,headland,straits,fountainhead,point,head,principal,caput,read/write_head,drumhead,headspring,mind,psyche,question,capitulum,pass,heading,chief,headway,brain,nous,school_principal,promontory,foreland,forefront,head_teacher,oral_sex,header,head_word</rdfs:comment>
        <rdfs:comment xml:lang="importstatement">edu.kit.ipd.ev3.IRobo</rdfs:comment>
        <rdfs:comment xml:lang="synonym">lift: cabbage,nobble,revoke,overturn,bring_up,go_up,hoist,rear,snarf,hook,come_up,move_up,raise,vacate,sneak,elevate,face-lift,repeal,rescind,filch,pinch,uprise,arise,abstract,get_up,reverse,plagiarise,purloin,countermand,plagiarize,annul,rustle,swipe,airlift,lift,pilfer,rise,wind</rdfs:comment>
        <rdfs:comment xml:lang="callstatement">liftHead</rdfs:comment>
        <rdfs:label xml:lang="en">liftHead</rdfs:label>
    </owl:NamedIndividual>
    


    <!-- Optional[http://www.semanticweb.org/team3/robo-ontology-0]/#long -->

    <owl:NamedIndividual rdf:about="Optional[http://www.semanticweb.org/team3/robo-ontology-0]/#long">
        <rdf:type rdf:resource="http://www.semanticweb.org/team3/robo-ontology-0#DataType"/>
        <rdfs:comment xml:lang="synonym">long:</rdfs:comment>
    </owl:NamedIndividual>
    


    <!-- Optional[http://www.semanticweb.org/team3/robo-ontology-0]/#look_6dbb4241_e4ae_4224_8a49_788d52a33877 -->

    <owl:NamedIndividual rdf:about="Optional[http://www.semanticweb.org/team3/robo-ontology-0]/#look_6dbb4241_e4ae_4224_8a49_788d52a33877">
        <rdf:type rdf:resource="http://www.semanticweb.org/team3/robo-ontology-0#Method"/>
        <hasParameter rdf:resource="Optional[http://www.semanticweb.org/team3/robo-ontology-0]/#direction_30496b80_b00f_4f70_809f_fdd7032448e8"/>
        <rdfs:comment xml:lang="importstatement">edu.kit.ipd.ev3.IRobo</rdfs:comment>
        <rdfs:comment xml:lang="callstatement">look</rdfs:comment>
        <rdfs:comment xml:lang="synonym">look: wait,attend,depend,count,look,seem,bet,appear,expect,search,face,see,bank,rely,take_care,await,front,calculate,reckon,swear</rdfs:comment>
        <rdfs:label xml:lang="en">look</rdfs:label>
    </owl:NamedIndividual>
    


    <!-- Optional[http://www.semanticweb.org/team3/robo-ontology-0]/#lowerHead_8d10f90b_e0aa_4647_87a3_5ff910ed72f3 -->

    <owl:NamedIndividual rdf:about="Optional[http://www.semanticweb.org/team3/robo-ontology-0]/#lowerHead_8d10f90b_e0aa_4647_87a3_5ff910ed72f3">
        <rdf:type rdf:resource="http://www.semanticweb.org/team3/robo-ontology-0#Method"/>
        <rdfs:comment xml:lang="synonym">Head: top_dog,headland,straits,fountainhead,point,head,principal,caput,read/write_head,drumhead,headspring,mind,psyche,question,capitulum,pass,heading,chief,headway,brain,nous,school_principal,promontory,foreland,forefront,head_teacher,oral_sex,header,head_word</rdfs:comment>
        <rdfs:comment xml:lang="importstatement">edu.kit.ipd.ev3.IRobo</rdfs:comment>
        <rdfs:comment xml:lang="synonym">lower: get_down,lour,bring_down,glower,turn_down,let_down,lower,take_down,frown,depress</rdfs:comment>
        <rdfs:comment xml:lang="callstatement">lowerHead</rdfs:comment>
        <rdfs:label xml:lang="en">lowerHead</rdfs:label>
    </owl:NamedIndividual>
    


    <!-- Optional[http://www.semanticweb.org/team3/robo-ontology-0]/#makeTowardsObject_408abcce_baac_479e_aa3f_d1ddbdc039ca -->

    <owl:NamedIndividual rdf:about="Optional[http://www.semanticweb.org/team3/robo-ontology-0]/#makeTowardsObject_408abcce_baac_479e_aa3f_d1ddbdc039ca">
        <rdf:type rdf:resource="http://www.semanticweb.org/team3/robo-ontology-0#Method"/>
        <hasParameter rdf:resource="Optional[http://www.semanticweb.org/team3/robo-ontology-0]/#object_12d6ddd0_92dd_4357_9b09_9d809fa77828"/>
        <rdfs:comment xml:lang="synonym">Towards:</rdfs:comment>
        <rdfs:comment xml:lang="importstatement">edu.kit.ipd.ev3.IRobo</rdfs:comment>
        <rdfs:comment xml:lang="synonym">make: stool,prepare,reach,do,construct,get_to,pretend,arrive_at,hold,nominate,score,pee,hit,pass_water,fix,create,attain,relieve_oneself,realize,give,work,constitute,make_up,piss,stimulate,establish,make_believe,take_in,take,induce,ca-ca,name,progress_to,spend_a_penny,puddle,lay_down,cause,gain,bring_in,ready,wee,get,have,defecate,pull_in,take_a_shit,make,wee-wee,cook,piddle,clear,draw,pee-pee,urinate,produce,crap,take_a_leak,take_a_crap,realise,form,build,throw,shit,earn,micturate,make_water,seduce</rdfs:comment>
        <rdfs:comment xml:lang="callstatement">makeTowardsObject</rdfs:comment>
        <rdfs:label xml:lang="en">makeTowardsObject</rdfs:label>
    </owl:NamedIndividual>
    


    <!-- Optional[http://www.semanticweb.org/team3/robo-ontology-0]/#medium -->

    <owl:NamedIndividual rdf:about="Optional[http://www.semanticweb.org/team3/robo-ontology-0]/#medium">
        <rdf:type rdf:resource="http://www.semanticweb.org/team3/robo-ontology-0#Value"/>
        <rdfs:comment xml:lang="callstatement">MEDIUM</rdfs:comment>
        <rdfs:comment xml:lang="importstatement">edu.kit.ipd.ev3.enums.Speed</rdfs:comment>
        <rdfs:comment xml:lang="synonym">medium: average,intermediate,medium</rdfs:comment>
    </owl:NamedIndividual>
    


    <!-- Optional[http://www.semanticweb.org/team3/robo-ontology-0]/#moveHead_066f8b00_afb5_4294_932e_7d2b6affeee1 -->

    <owl:NamedIndividual rdf:about="Optional[http://www.semanticweb.org/team3/robo-ontology-0]/#moveHead_066f8b00_afb5_4294_932e_7d2b6affeee1">
        <rdf:type rdf:resource="http://www.semanticweb.org/team3/robo-ontology-0#Method"/>
        <hasParameter rdf:resource="Optional[http://www.semanticweb.org/team3/robo-ontology-0]/#direction_c6aeeb65_4287_41e0_8fec_371521e2d3e7"/>
        <rdfs:comment xml:lang="synonym">Head: top_dog,headland,straits,fountainhead,point,head,principal,caput,read/write_head,drumhead,headspring,mind,psyche,question,capitulum,pass,heading,chief,headway,brain,nous,school_principal,promontory,foreland,forefront,head_teacher,oral_sex,header,head_word</rdfs:comment>
        <rdfs:comment xml:lang="importstatement">edu.kit.ipd.ev3.IRobo</rdfs:comment>
        <rdfs:comment xml:lang="synonym">move: move,proceed,displace,affect,make_a_motion,strike,go,be_active,actuate,run,impress,locomote,act,propel,incite,motivate,travel,prompt</rdfs:comment>
        <rdfs:comment xml:lang="callstatement">moveHead</rdfs:comment>
        <rdfs:label xml:lang="en">moveHead</rdfs:label>
    </owl:NamedIndividual>
    


    <!-- Optional[http://www.semanticweb.org/team3/robo-ontology-0]/#moveUntil_cc47bc97_a95a_4277_83a7_1302c927988e -->

    <owl:NamedIndividual rdf:about="Optional[http://www.semanticweb.org/team3/robo-ontology-0]/#moveUntil_cc47bc97_a95a_4277_83a7_1302c927988e">
        <rdf:type rdf:resource="http://www.semanticweb.org/team3/robo-ontology-0#Method"/>
        <hasParameter rdf:resource="Optional[http://www.semanticweb.org/team3/robo-ontology-0]/#condition_ac983e93_487b_498b_9ea0_c1f1009739fd"/>
        <hasParameter rdf:resource="Optional[http://www.semanticweb.org/team3/robo-ontology-0]/#dir_3e10eb90_4969_4f3a_a5ef_d45c1f342e86"/>
        <rdfs:comment xml:lang="importstatement">edu.kit.ipd.ev3.IRobo</rdfs:comment>
        <rdfs:comment xml:lang="synonym">move: move,proceed,displace,affect,make_a_motion,strike,go,be_active,actuate,run,impress,locomote,act,propel,incite,motivate,travel,prompt</rdfs:comment>
        <rdfs:comment xml:lang="callstatement">moveUntil</rdfs:comment>
        <rdfs:label xml:lang="en">moveUntil</rdfs:label>
    </owl:NamedIndividual>
    


    <!-- Optional[http://www.semanticweb.org/team3/robo-ontology-0]/#moveUntil_ff3749ee_8ffb_4dd6_bb74_9a9f570def7c -->

    <owl:NamedIndividual rdf:about="Optional[http://www.semanticweb.org/team3/robo-ontology-0]/#moveUntil_ff3749ee_8ffb_4dd6_bb74_9a9f570def7c">
        <rdf:type rdf:resource="http://www.semanticweb.org/team3/robo-ontology-0#Method"/>
        <hasParameter rdf:resource="Optional[http://www.semanticweb.org/team3/robo-ontology-0]/#condition_c26dbe68_f60f_4635_b13f_e238d4432256"/>
        <hasParameter rdf:resource="Optional[http://www.semanticweb.org/team3/robo-ontology-0]/#dir_17ceb3d5_f0c6_4c6c_bf2c_55af1027d5b3"/>
        <hasParameter rdf:resource="Optional[http://www.semanticweb.org/team3/robo-ontology-0]/#speed_652ac91f_9e86_4b93_824f_220c9a07202b"/>
        <rdfs:comment xml:lang="importstatement">edu.kit.ipd.ev3.IRobo</rdfs:comment>
        <rdfs:comment xml:lang="synonym">move: move,proceed,displace,affect,make_a_motion,strike,go,be_active,actuate,run,impress,locomote,act,propel,incite,motivate,travel,prompt</rdfs:comment>
        <rdfs:comment xml:lang="callstatement">moveUntil</rdfs:comment>
        <rdfs:label xml:lang="en">moveUntil</rdfs:label>
    </owl:NamedIndividual>
    


    <!-- Optional[http://www.semanticweb.org/team3/robo-ontology-0]/#move_1b2b5e11_c82c_4937_8850_c3d59e2c1c15 -->

    <owl:NamedIndividual rdf:about="Optional[http://www.semanticweb.org/team3/robo-ontology-0]/#move_1b2b5e11_c82c_4937_8850_c3d59e2c1c15">
        <rdf:type rdf:resource="http://www.semanticweb.org/team3/robo-ontology-0#Method"/>
        <hasParameter rdf:resource="Optional[http://www.semanticweb.org/team3/robo-ontology-0]/#dir_9a14702b_2d5e_4650_a755_934ab436b793"/>
        <hasParameter rdf:resource="Optional[http://www.semanticweb.org/team3/robo-ontology-0]/#time_379b6aea_733e_4f0a_9bbd_26ba641409c5"/>
        <rdfs:comment xml:lang="importstatement">edu.kit.ipd.ev3.IRobo</rdfs:comment>
        <rdfs:comment xml:lang="callstatement">move</rdfs:comment>
        <rdfs:comment xml:lang="synonym">move: move,proceed,displace,affect,make_a_motion,strike,go,be_active,actuate,run,impress,locomote,act,propel,incite,motivate,travel,prompt</rdfs:comment>
        <rdfs:label xml:lang="en">move</rdfs:label>
    </owl:NamedIndividual>
    


    <!-- Optional[http://www.semanticweb.org/team3/robo-ontology-0]/#move_7815995a_f151_4e53_acd7_3770ade9e721 -->

    <owl:NamedIndividual rdf:about="Optional[http://www.semanticweb.org/team3/robo-ontology-0]/#move_7815995a_f151_4e53_acd7_3770ade9e721">
        <rdf:type rdf:resource="http://www.semanticweb.org/team3/robo-ontology-0#Method"/>
        <hasParameter rdf:resource="Optional[http://www.semanticweb.org/team3/robo-ontology-0]/#dir_2650cea4_8219_42ad_8c2d_32aa10504a2e"/>
        <hasParameter rdf:resource="Optional[http://www.semanticweb.org/team3/robo-ontology-0]/#speed_1f5ae49e_945e_4455_b13f_8f70f8a30647"/>
        <hasParameter rdf:resource="Optional[http://www.semanticweb.org/team3/robo-ontology-0]/#time_46b7b4f4_e3dd_424d_8d16_797b1c201f13"/>
        <rdfs:comment xml:lang="importstatement">edu.kit.ipd.ev3.IRobo</rdfs:comment>
        <rdfs:comment xml:lang="callstatement">move</rdfs:comment>
        <rdfs:comment xml:lang="synonym">move: move,proceed,displace,affect,make_a_motion,strike,go,be_active,actuate,run,impress,locomote,act,propel,incite,motivate,travel,prompt</rdfs:comment>
        <rdfs:label xml:lang="en">move</rdfs:label>
    </owl:NamedIndividual>
    


    <!-- Optional[http://www.semanticweb.org/team3/robo-ontology-0]/#move_a0eb6a93_ee54_4680_8963_d6249cb69791 -->

    <owl:NamedIndividual rdf:about="Optional[http://www.semanticweb.org/team3/robo-ontology-0]/#move_a0eb6a93_ee54_4680_8963_d6249cb69791">
        <rdf:type rdf:resource="http://www.semanticweb.org/team3/robo-ontology-0#Method"/>
        <hasParameter rdf:resource="Optional[http://www.semanticweb.org/team3/robo-ontology-0]/#dir_d2165658_484a_4759_89b6_a53ec9c2e631"/>
        <rdfs:comment xml:lang="importstatement">edu.kit.ipd.ev3.IRobo</rdfs:comment>
        <rdfs:comment xml:lang="callstatement">move</rdfs:comment>
        <rdfs:comment xml:lang="synonym">move: move,proceed,displace,affect,make_a_motion,strike,go,be_active,actuate,run,impress,locomote,act,propel,incite,motivate,travel,prompt</rdfs:comment>
        <rdfs:label xml:lang="en">move</rdfs:label>
    </owl:NamedIndividual>
    


    <!-- Optional[http://www.semanticweb.org/team3/robo-ontology-0]/#move_f06a062a_952c_4f07_9752_69c55b0140be -->

    <owl:NamedIndividual rdf:about="Optional[http://www.semanticweb.org/team3/robo-ontology-0]/#move_f06a062a_952c_4f07_9752_69c55b0140be">
        <rdf:type rdf:resource="http://www.semanticweb.org/team3/robo-ontology-0#Method"/>
        <hasParameter rdf:resource="Optional[http://www.semanticweb.org/team3/robo-ontology-0]/#dir_7730cef1_1bed_43f3_8217_ab397f9f5aaa"/>
        <hasParameter rdf:resource="Optional[http://www.semanticweb.org/team3/robo-ontology-0]/#length_aa148b58_7162_4931_a0cf_af3a607ff503"/>
        <rdfs:comment xml:lang="importstatement">edu.kit.ipd.ev3.IRobo</rdfs:comment>
        <rdfs:comment xml:lang="callstatement">move</rdfs:comment>
        <rdfs:comment xml:lang="synonym">move: move,proceed,displace,affect,make_a_motion,strike,go,be_active,actuate,run,impress,locomote,act,propel,incite,motivate,travel,prompt</rdfs:comment>
        <rdfs:label xml:lang="en">move</rdfs:label>
    </owl:NamedIndividual>
    


    <!-- Optional[http://www.semanticweb.org/team3/robo-ontology-0]/#move_fdd5345b_7ce2_4000_a81b_99529d0fd6db -->

    <owl:NamedIndividual rdf:about="Optional[http://www.semanticweb.org/team3/robo-ontology-0]/#move_fdd5345b_7ce2_4000_a81b_99529d0fd6db">
        <rdf:type rdf:resource="http://www.semanticweb.org/team3/robo-ontology-0#Method"/>
        <hasParameter rdf:resource="Optional[http://www.semanticweb.org/team3/robo-ontology-0]/#dir_2882212f_ba3e_4547_a62c_fcf356ce5ca3"/>
        <hasParameter rdf:resource="Optional[http://www.semanticweb.org/team3/robo-ontology-0]/#length_1aae939b_0bc1_4a19_be30_1ab2a44dc159"/>
        <hasParameter rdf:resource="Optional[http://www.semanticweb.org/team3/robo-ontology-0]/#speed_b81f497f_f334_4333_a068_442b5d533c4b"/>
        <rdfs:comment xml:lang="importstatement">edu.kit.ipd.ev3.IRobo</rdfs:comment>
        <rdfs:comment xml:lang="callstatement">move</rdfs:comment>
        <rdfs:comment xml:lang="synonym">move: move,proceed,displace,affect,make_a_motion,strike,go,be_active,actuate,run,impress,locomote,act,propel,incite,motivate,travel,prompt</rdfs:comment>
        <rdfs:label xml:lang="en">move</rdfs:label>
    </owl:NamedIndividual>
    


    <!-- Optional[http://www.semanticweb.org/team3/robo-ontology-0]/#object_12d6ddd0_92dd_4357_9b09_9d809fa77828 -->

    <owl:NamedIndividual rdf:about="Optional[http://www.semanticweb.org/team3/robo-ontology-0]/#object_12d6ddd0_92dd_4357_9b09_9d809fa77828">
        <rdf:type rdf:resource="http://www.semanticweb.org/team3/robo-ontology-0#Parameter"/>
        <ofDataType rdf:resource="http://www.semanticweb.org/team3/robo-ontology-0#Object"/>
        <rdfs:comment xml:lang="pos">0</rdfs:comment>
        <rdfs:label xml:lang="en">object</rdfs:label>
    </owl:NamedIndividual>
    


    <!-- Optional[http://www.semanticweb.org/team3/robo-ontology-0]/#object_181d35ea_223f_4cdf_b809_330916e585bb -->

    <owl:NamedIndividual rdf:about="Optional[http://www.semanticweb.org/team3/robo-ontology-0]/#object_181d35ea_223f_4cdf_b809_330916e585bb">
        <rdf:type rdf:resource="http://www.semanticweb.org/team3/robo-ontology-0#Parameter"/>
        <ofDataType rdf:resource="http://www.semanticweb.org/team3/robo-ontology-0#Object"/>
        <rdfs:comment xml:lang="pos">0</rdfs:comment>
        <rdfs:label xml:lang="en">object</rdfs:label>
    </owl:NamedIndividual>
    


    <!-- Optional[http://www.semanticweb.org/team3/robo-ontology-0]/#object_516c2e4e_acb1_403f_ae09_4a46a22c7ec2 -->

    <owl:NamedIndividual rdf:about="Optional[http://www.semanticweb.org/team3/robo-ontology-0]/#object_516c2e4e_acb1_403f_ae09_4a46a22c7ec2">
        <rdf:type rdf:resource="http://www.semanticweb.org/team3/robo-ontology-0#Parameter"/>
        <ofDataType rdf:resource="http://www.semanticweb.org/team3/robo-ontology-0#Object"/>
        <rdfs:comment xml:lang="pos">0</rdfs:comment>
        <rdfs:label xml:lang="en">object</rdfs:label>
    </owl:NamedIndividual>
    


    <!-- Optional[http://www.semanticweb.org/team3/robo-ontology-0]/#object_52a6de59_263a_4cfb_aa28_c86b12869ee7 -->

    <owl:NamedIndividual rdf:about="Optional[http://www.semanticweb.org/team3/robo-ontology-0]/#object_52a6de59_263a_4cfb_aa28_c86b12869ee7">
        <rdf:type rdf:resource="http://www.semanticweb.org/team3/robo-ontology-0#Parameter"/>
        <ofDataType rdf:resource="http://www.semanticweb.org/team3/robo-ontology-0#Object"/>
        <rdfs:comment xml:lang="pos">0</rdfs:comment>
        <rdfs:label xml:lang="en">object</rdfs:label>
    </owl:NamedIndividual>
    


    <!-- Optional[http://www.semanticweb.org/team3/robo-ontology-0]/#object_8e5c825e_02b6_40bc_8b54_0f165afa4201 -->

    <owl:NamedIndividual rdf:about="Optional[http://www.semanticweb.org/team3/robo-ontology-0]/#object_8e5c825e_02b6_40bc_8b54_0f165afa4201">
        <rdf:type rdf:resource="http://www.semanticweb.org/team3/robo-ontology-0#Parameter"/>
        <ofDataType rdf:resource="http://www.semanticweb.org/team3/robo-ontology-0#Object"/>
        <rdfs:comment xml:lang="pos">0</rdfs:comment>
        <rdfs:label xml:lang="en">object</rdfs:label>
    </owl:NamedIndividual>
    


    <!-- Optional[http://www.semanticweb.org/team3/robo-ontology-0]/#object_af319d4f_f219_4895_8cde_63607b4334c2 -->

    <owl:NamedIndividual rdf:about="Optional[http://www.semanticweb.org/team3/robo-ontology-0]/#object_af319d4f_f219_4895_8cde_63607b4334c2">
        <rdf:type rdf:resource="http://www.semanticweb.org/team3/robo-ontology-0#Parameter"/>
        <ofDataType rdf:resource="http://www.semanticweb.org/team3/robo-ontology-0#Object"/>
        <rdfs:comment xml:lang="pos">0</rdfs:comment>
        <rdfs:label xml:lang="en">object</rdfs:label>
    </owl:NamedIndividual>
    


    <!-- Optional[http://www.semanticweb.org/team3/robo-ontology-0]/#object_b117c778_2f59_4e4e_b69b_f7dd8e3a4e21 -->

    <owl:NamedIndividual rdf:about="Optional[http://www.semanticweb.org/team3/robo-ontology-0]/#object_b117c778_2f59_4e4e_b69b_f7dd8e3a4e21">
        <rdf:type rdf:resource="http://www.semanticweb.org/team3/robo-ontology-0#Parameter"/>
        <ofDataType rdf:resource="http://www.semanticweb.org/team3/robo-ontology-0#Object"/>
        <rdfs:comment xml:lang="pos">0</rdfs:comment>
        <rdfs:label xml:lang="en">object</rdfs:label>
    </owl:NamedIndividual>
    


    <!-- Optional[http://www.semanticweb.org/team3/robo-ontology-0]/#playHalloweenTheme_03b52809_060c_4641_bad6_7583e56ad53e -->

    <owl:NamedIndividual rdf:about="Optional[http://www.semanticweb.org/team3/robo-ontology-0]/#playHalloweenTheme_03b52809_060c_4641_bad6_7583e56ad53e">
        <rdf:type rdf:resource="http://www.semanticweb.org/team3/robo-ontology-0#Method"/>
        <rdfs:comment xml:lang="synonym">Halloween: Hallowe&apos;en,Halloween,Allhallows_Eve</rdfs:comment>
        <rdfs:comment xml:lang="synonym">Theme: radical,subject,idea,melodic_theme,root_word,paper,musical_theme,composition,root,report,topic,theme,motif,base,stem</rdfs:comment>
        <rdfs:comment xml:lang="importstatement">edu.kit.ipd.ev3.IRobo</rdfs:comment>
        <rdfs:comment xml:lang="synonym">play: play,roleplay,diddle,work,bring,run,playact,encounter,recreate,act_as,bet,wager,dally,act,meet,flirt,wreak,make_for,fiddle,spiel,take_on,trifle,represent,toy</rdfs:comment>
        <rdfs:comment xml:lang="callstatement">playHalloweenTheme</rdfs:comment>
        <rdfs:label xml:lang="en">playHalloweenTheme</rdfs:label>
    </owl:NamedIndividual>
    


    <!-- Optional[http://www.semanticweb.org/team3/robo-ontology-0]/#quarter -->

    <owl:NamedIndividual rdf:about="Optional[http://www.semanticweb.org/team3/robo-ontology-0]/#quarter">
        <rdf:type rdf:resource="http://www.semanticweb.org/team3/robo-ontology-0#Value"/>
        <rdfs:comment xml:lang="callstatement">QUARTER</rdfs:comment>
        <rdfs:comment xml:lang="importstatement">edu.kit.ipd.ev3.enums.Revolution</rdfs:comment>
        <rdfs:comment xml:lang="synonym">quarter:</rdfs:comment>
    </owl:NamedIndividual>
    


    <!-- Optional[http://www.semanticweb.org/team3/robo-ontology-0]/#red -->

    <owl:NamedIndividual rdf:about="Optional[http://www.semanticweb.org/team3/robo-ontology-0]/#red">
        <rdf:type rdf:resource="http://www.semanticweb.org/team3/robo-ontology-0#Value"/>
        <rdfs:comment xml:lang="callstatement">RED</rdfs:comment>
        <rdfs:comment xml:lang="importstatement">edu.kit.ipd.ev3.enums.Color</rdfs:comment>
        <rdfs:comment xml:lang="synonym">red: cherry,violent,cherry-red,ruby-red,ruddy,reddened,flushed,carmine,ruby,red,scarlet,crimson,blood-red,reddish,cerise,red-faced</rdfs:comment>
    </owl:NamedIndividual>
    


    <!-- Optional[http://www.semanticweb.org/team3/robo-ontology-0]/#release_23fd61bc_a93a_4590_b9af_c46197f9fdc9 -->

    <owl:NamedIndividual rdf:about="Optional[http://www.semanticweb.org/team3/robo-ontology-0]/#release_23fd61bc_a93a_4590_b9af_c46197f9fdc9">
        <rdf:type rdf:resource="http://www.semanticweb.org/team3/robo-ontology-0#Method"/>
        <hasParameter rdf:resource="Optional[http://www.semanticweb.org/team3/robo-ontology-0]/#object_181d35ea_223f_4cdf_b809_330916e585bb"/>
        <rdfs:comment xml:lang="importstatement">edu.kit.ipd.ev3.IRobo</rdfs:comment>
        <rdfs:comment xml:lang="callstatement">release</rdfs:comment>
        <rdfs:comment xml:lang="synonym">release: expel,issue,release,exhaust,turn,unfreeze,liberate,let_go_of,put_out,unloose,eject,unblock,bring_out,give_up,publish,loose,discharge,relinquish,unloosen,secrete,let_go,free,resign</rdfs:comment>
        <rdfs:label xml:lang="en">release</rdfs:label>
    </owl:NamedIndividual>
    


    <!-- Optional[http://www.semanticweb.org/team3/robo-ontology-0]/#rev_24a66090_a410_4a79_a000_07f20e71b05f -->

    <owl:NamedIndividual rdf:about="Optional[http://www.semanticweb.org/team3/robo-ontology-0]/#rev_24a66090_a410_4a79_a000_07f20e71b05f">
        <rdf:type rdf:resource="http://www.semanticweb.org/team3/robo-ontology-0#Parameter"/>
        <ofDataType rdf:resource="Optional[http://www.semanticweb.org/team3/robo-ontology-0]/#Revolution"/>
        <rdfs:comment xml:lang="pos">1</rdfs:comment>
        <rdfs:label xml:lang="en">rev</rdfs:label>
    </owl:NamedIndividual>
    


    <!-- Optional[http://www.semanticweb.org/team3/robo-ontology-0]/#rev_4c1bc855_4541_46de_af2a_163088812227 -->

    <owl:NamedIndividual rdf:about="Optional[http://www.semanticweb.org/team3/robo-ontology-0]/#rev_4c1bc855_4541_46de_af2a_163088812227">
        <rdf:type rdf:resource="http://www.semanticweb.org/team3/robo-ontology-0#Parameter"/>
        <ofDataType rdf:resource="Optional[http://www.semanticweb.org/team3/robo-ontology-0]/#Revolution"/>
        <rdfs:comment xml:lang="pos">0</rdfs:comment>
        <rdfs:label xml:lang="en">rev</rdfs:label>
    </owl:NamedIndividual>
    


    <!-- Optional[http://www.semanticweb.org/team3/robo-ontology-0]/#rev_8700ae64_ffb9_45ed_8d20_0f865c4a96c0 -->

    <owl:NamedIndividual rdf:about="Optional[http://www.semanticweb.org/team3/robo-ontology-0]/#rev_8700ae64_ffb9_45ed_8d20_0f865c4a96c0">
        <rdf:type rdf:resource="http://www.semanticweb.org/team3/robo-ontology-0#Parameter"/>
        <ofDataType rdf:resource="Optional[http://www.semanticweb.org/team3/robo-ontology-0]/#Revolution"/>
        <rdfs:comment xml:lang="pos">1</rdfs:comment>
        <rdfs:label xml:lang="en">rev</rdfs:label>
    </owl:NamedIndividual>
    


    <!-- Optional[http://www.semanticweb.org/team3/robo-ontology-0]/#rev_8f4d3bfc_5595_4ba3_8863_8e88ea42a574 -->

    <owl:NamedIndividual rdf:about="Optional[http://www.semanticweb.org/team3/robo-ontology-0]/#rev_8f4d3bfc_5595_4ba3_8863_8e88ea42a574">
        <rdf:type rdf:resource="http://www.semanticweb.org/team3/robo-ontology-0#Parameter"/>
        <ofDataType rdf:resource="Optional[http://www.semanticweb.org/team3/robo-ontology-0]/#Revolution"/>
        <rdfs:comment xml:lang="pos">0</rdfs:comment>
        <rdfs:label xml:lang="en">rev</rdfs:label>
    </owl:NamedIndividual>
    


    <!-- Optional[http://www.semanticweb.org/team3/robo-ontology-0]/#right -->

    <owl:NamedIndividual rdf:about="Optional[http://www.semanticweb.org/team3/robo-ontology-0]/#right">
        <rdf:type rdf:resource="http://www.semanticweb.org/team3/robo-ontology-0#Value"/>
        <rdfs:comment xml:lang="callstatement">RIGHT</rdfs:comment>
        <rdfs:comment xml:lang="importstatement">edu.kit.ipd.ev3.enums.Direction</rdfs:comment>
        <rdfs:comment xml:lang="synonym">right: correct,right-hand,one,proper,ripe,right,veracious,good</rdfs:comment>
    </owl:NamedIndividual>
    


    <!-- Optional[http://www.semanticweb.org/team3/robo-ontology-0]/#sayGoodbye_29e06e21_df38_4ac0_8b26_fe3580981233 -->

    <owl:NamedIndividual rdf:about="Optional[http://www.semanticweb.org/team3/robo-ontology-0]/#sayGoodbye_29e06e21_df38_4ac0_8b26_fe3580981233">
        <rdf:type rdf:resource="http://www.semanticweb.org/team3/robo-ontology-0#Method"/>
        <rdfs:comment xml:lang="synonym">Goodbye: goodby,goodbye,sayonara,cheerio,bye-bye,adios,bye,good-by,adieu,auf_wiedersehen,good-bye,au_revoir,arrivederci,so_long,good_day</rdfs:comment>
        <rdfs:comment xml:lang="importstatement">edu.kit.ipd.ev3.IRobo</rdfs:comment>
        <rdfs:comment xml:lang="synonym">say: sound_out,read,tell,allege,articulate,say,enjoin,suppose,aver,enunciate,state,pronounce,enounce,order</rdfs:comment>
        <rdfs:comment xml:lang="callstatement">sayGoodbye</rdfs:comment>
        <rdfs:label xml:lang="en">sayGoodbye</rdfs:label>
    </owl:NamedIndividual>
    


    <!-- Optional[http://www.semanticweb.org/team3/robo-ontology-0]/#sing_e7266fd2_7104_4bc6_b8ba_595c3c4882a9 -->

    <owl:NamedIndividual rdf:about="Optional[http://www.semanticweb.org/team3/robo-ontology-0]/#sing_e7266fd2_7104_4bc6_b8ba_595c3c4882a9">
        <rdf:type rdf:resource="http://www.semanticweb.org/team3/robo-ontology-0#Method"/>
        <rdfs:comment xml:lang="importstatement">edu.kit.ipd.ev3.IRobo</rdfs:comment>
        <rdfs:comment xml:lang="callstatement">sing</rdfs:comment>
        <rdfs:comment xml:lang="synonym">sing: spill_the_beans,blab,blab_out,babble,peach,whistle,tattle,sing,talk,let_the_cat_out_of_the_bag,babble_out</rdfs:comment>
        <rdfs:label xml:lang="en">sing</rdfs:label>
    </owl:NamedIndividual>
    


    <!-- Optional[http://www.semanticweb.org/team3/robo-ontology-0]/#slow -->

    <owl:NamedIndividual rdf:about="Optional[http://www.semanticweb.org/team3/robo-ontology-0]/#slow">
        <rdf:type rdf:resource="http://www.semanticweb.org/team3/robo-ontology-0#Value"/>
        <rdfs:comment xml:lang="callstatement">SLOW</rdfs:comment>
        <rdfs:comment xml:lang="importstatement">edu.kit.ipd.ev3.enums.Speed</rdfs:comment>
        <rdfs:comment xml:lang="synonym">slow: obtuse,deadening,irksome,dim,dumb,tedious,sluggish,dense,ho-hum,boring,slow,wearisome,tiresome,dull</rdfs:comment>
    </owl:NamedIndividual>
    


    <!-- Optional[http://www.semanticweb.org/team3/robo-ontology-0]/#slowest -->

    <owl:NamedIndividual rdf:about="Optional[http://www.semanticweb.org/team3/robo-ontology-0]/#slowest">
        <rdf:type rdf:resource="http://www.semanticweb.org/team3/robo-ontology-0#Value"/>
        <rdfs:comment xml:lang="callstatement">SLOWEST</rdfs:comment>
        <rdfs:comment xml:lang="importstatement">edu.kit.ipd.ev3.enums.Speed</rdfs:comment>
        <rdfs:comment xml:lang="synonym">slowest:</rdfs:comment>
    </owl:NamedIndividual>
    


    <!-- Optional[http://www.semanticweb.org/team3/robo-ontology-0]/#speed_1f5ae49e_945e_4455_b13f_8f70f8a30647 -->

    <owl:NamedIndividual rdf:about="Optional[http://www.semanticweb.org/team3/robo-ontology-0]/#speed_1f5ae49e_945e_4455_b13f_8f70f8a30647">
        <rdf:type rdf:resource="http://www.semanticweb.org/team3/robo-ontology-0#Parameter"/>
        <ofDataType rdf:resource="Optional[http://www.semanticweb.org/team3/robo-ontology-0]/#Speed"/>
        <rdfs:comment xml:lang="pos">2</rdfs:comment>
        <rdfs:label xml:lang="en">speed</rdfs:label>
    </owl:NamedIndividual>
    


    <!-- Optional[http://www.semanticweb.org/team3/robo-ontology-0]/#speed_3163d405_0aae_4b21_99ff_11acf5012130 -->

    <owl:NamedIndividual rdf:about="Optional[http://www.semanticweb.org/team3/robo-ontology-0]/#speed_3163d405_0aae_4b21_99ff_11acf5012130">
        <rdf:type rdf:resource="http://www.semanticweb.org/team3/robo-ontology-0#Parameter"/>
        <ofDataType rdf:resource="Optional[http://www.semanticweb.org/team3/robo-ontology-0]/#Speed"/>
        <rdfs:comment xml:lang="pos">2</rdfs:comment>
        <rdfs:label xml:lang="en">speed</rdfs:label>
    </owl:NamedIndividual>
    


    <!-- Optional[http://www.semanticweb.org/team3/robo-ontology-0]/#speed_380373bb_b428_4a6c_b553_779f56c0c983 -->

    <owl:NamedIndividual rdf:about="Optional[http://www.semanticweb.org/team3/robo-ontology-0]/#speed_380373bb_b428_4a6c_b553_779f56c0c983">
        <rdf:type rdf:resource="http://www.semanticweb.org/team3/robo-ontology-0#Parameter"/>
        <ofDataType rdf:resource="Optional[http://www.semanticweb.org/team3/robo-ontology-0]/#Speed"/>
        <rdfs:comment xml:lang="pos">0</rdfs:comment>
        <rdfs:label xml:lang="en">speed</rdfs:label>
    </owl:NamedIndividual>
    


    <!-- Optional[http://www.semanticweb.org/team3/robo-ontology-0]/#speed_5bff6444_195d_489a_8c6d_99d9aa8ae08b -->

    <owl:NamedIndividual rdf:about="Optional[http://www.semanticweb.org/team3/robo-ontology-0]/#speed_5bff6444_195d_489a_8c6d_99d9aa8ae08b">
        <rdf:type rdf:resource="http://www.semanticweb.org/team3/robo-ontology-0#Parameter"/>
        <ofDataType rdf:resource="Optional[http://www.semanticweb.org/team3/robo-ontology-0]/#Speed"/>
        <rdfs:comment xml:lang="pos">1</rdfs:comment>
        <rdfs:label xml:lang="en">speed</rdfs:label>
    </owl:NamedIndividual>
    


    <!-- Optional[http://www.semanticweb.org/team3/robo-ontology-0]/#speed_652ac91f_9e86_4b93_824f_220c9a07202b -->

    <owl:NamedIndividual rdf:about="Optional[http://www.semanticweb.org/team3/robo-ontology-0]/#speed_652ac91f_9e86_4b93_824f_220c9a07202b">
        <rdf:type rdf:resource="http://www.semanticweb.org/team3/robo-ontology-0#Parameter"/>
        <ofDataType rdf:resource="Optional[http://www.semanticweb.org/team3/robo-ontology-0]/#Speed"/>
        <rdfs:comment xml:lang="pos">1</rdfs:comment>
        <rdfs:label xml:lang="en">speed</rdfs:label>
    </owl:NamedIndividual>
    


    <!-- Optional[http://www.semanticweb.org/team3/robo-ontology-0]/#speed_839c7b48_927a_4a06_bbd3_24a364489f5b -->

    <owl:NamedIndividual rdf:about="Optional[http://www.semanticweb.org/team3/robo-ontology-0]/#speed_839c7b48_927a_4a06_bbd3_24a364489f5b">
        <rdf:type rdf:resource="http://www.semanticweb.org/team3/robo-ontology-0#Parameter"/>
        <ofDataType rdf:resource="Optional[http://www.semanticweb.org/team3/robo-ontology-0]/#Speed"/>
        <rdfs:comment xml:lang="pos">1</rdfs:comment>
        <rdfs:label xml:lang="en">speed</rdfs:label>
    </owl:NamedIndividual>
    


    <!-- Optional[http://www.semanticweb.org/team3/robo-ontology-0]/#speed_89664740_d918_4358_b515_992fd86b6143 -->

    <owl:NamedIndividual rdf:about="Optional[http://www.semanticweb.org/team3/robo-ontology-0]/#speed_89664740_d918_4358_b515_992fd86b6143">
        <rdf:type rdf:resource="http://www.semanticweb.org/team3/robo-ontology-0#Parameter"/>
        <ofDataType rdf:resource="Optional[http://www.semanticweb.org/team3/robo-ontology-0]/#Speed"/>
        <rdfs:comment xml:lang="pos">2</rdfs:comment>
        <rdfs:label xml:lang="en">speed</rdfs:label>
    </owl:NamedIndividual>
    


    <!-- Optional[http://www.semanticweb.org/team3/robo-ontology-0]/#speed_920277e4_7341_4e21_a0b8_84150fa97224 -->

    <owl:NamedIndividual rdf:about="Optional[http://www.semanticweb.org/team3/robo-ontology-0]/#speed_920277e4_7341_4e21_a0b8_84150fa97224">
        <rdf:type rdf:resource="http://www.semanticweb.org/team3/robo-ontology-0#Parameter"/>
        <ofDataType rdf:resource="Optional[http://www.semanticweb.org/team3/robo-ontology-0]/#Speed"/>
        <rdfs:comment xml:lang="pos">1</rdfs:comment>
        <rdfs:label xml:lang="en">speed</rdfs:label>
    </owl:NamedIndividual>
    


    <!-- Optional[http://www.semanticweb.org/team3/robo-ontology-0]/#speed_b81f497f_f334_4333_a068_442b5d533c4b -->

    <owl:NamedIndividual rdf:about="Optional[http://www.semanticweb.org/team3/robo-ontology-0]/#speed_b81f497f_f334_4333_a068_442b5d533c4b">
        <rdf:type rdf:resource="http://www.semanticweb.org/team3/robo-ontology-0#Parameter"/>
        <ofDataType rdf:resource="Optional[http://www.semanticweb.org/team3/robo-ontology-0]/#Speed"/>
        <rdfs:comment xml:lang="pos">2</rdfs:comment>
        <rdfs:label xml:lang="en">speed</rdfs:label>
    </owl:NamedIndividual>
    


    <!-- Optional[http://www.semanticweb.org/team3/robo-ontology-0]/#speed_e1d0e420_4dfb_4fe4_b44b_4a3644e6d36c -->

    <owl:NamedIndividual rdf:about="Optional[http://www.semanticweb.org/team3/robo-ontology-0]/#speed_e1d0e420_4dfb_4fe4_b44b_4a3644e6d36c">
        <rdf:type rdf:resource="http://www.semanticweb.org/team3/robo-ontology-0#Parameter"/>
        <ofDataType rdf:resource="Optional[http://www.semanticweb.org/team3/robo-ontology-0]/#Speed"/>
        <rdfs:comment xml:lang="pos">0</rdfs:comment>
        <rdfs:label xml:lang="en">speed</rdfs:label>
    </owl:NamedIndividual>
    


    <!-- Optional[http://www.semanticweb.org/team3/robo-ontology-0]/#speed_ecaafbbb_46d9_4303_968a_a64bc1029fab -->

    <owl:NamedIndividual rdf:about="Optional[http://www.semanticweb.org/team3/robo-ontology-0]/#speed_ecaafbbb_46d9_4303_968a_a64bc1029fab">
        <rdf:type rdf:resource="http://www.semanticweb.org/team3/robo-ontology-0#Parameter"/>
        <ofDataType rdf:resource="Optional[http://www.semanticweb.org/team3/robo-ontology-0]/#Speed"/>
        <rdfs:comment xml:lang="pos">2</rdfs:comment>
        <rdfs:label xml:lang="en">speed</rdfs:label>
    </owl:NamedIndividual>
    


    <!-- Optional[http://www.semanticweb.org/team3/robo-ontology-0]/#speed_f476e627_864c_41e2_9f24_deb1e70bd7d6 -->

    <owl:NamedIndividual rdf:about="Optional[http://www.semanticweb.org/team3/robo-ontology-0]/#speed_f476e627_864c_41e2_9f24_deb1e70bd7d6">
        <rdf:type rdf:resource="http://www.semanticweb.org/team3/robo-ontology-0#Parameter"/>
        <ofDataType rdf:resource="Optional[http://www.semanticweb.org/team3/robo-ontology-0]/#Speed"/>
        <rdfs:comment xml:lang="pos">1</rdfs:comment>
        <rdfs:label xml:lang="en">speed</rdfs:label>
    </owl:NamedIndividual>
    


    <!-- Optional[http://www.semanticweb.org/team3/robo-ontology-0]/#throwAway_e5d7fcb6_3209_41a4_b516_4e356c46d717 -->

    <owl:NamedIndividual rdf:about="Optional[http://www.semanticweb.org/team3/robo-ontology-0]/#throwAway_e5d7fcb6_3209_41a4_b516_4e356c46d717">
        <rdf:type rdf:resource="http://www.semanticweb.org/team3/robo-ontology-0#Method"/>
        <hasParameter rdf:resource="Optional[http://www.semanticweb.org/team3/robo-ontology-0]/#object_516c2e4e_acb1_403f_ae09_4a46a22c7ec2"/>
        <rdfs:comment xml:lang="synonym">Away: away,outside</rdfs:comment>
        <rdfs:comment xml:lang="importstatement">edu.kit.ipd.ev3.IRobo</rdfs:comment>
        <rdfs:comment xml:lang="synonym">throw: throw_away,drop,bemuse,shed,discombobulate,project,fox,switch,hold,cast,confuse,have,flip,make,give,fuddle,bewilder,contrive,confound,throw_off,shake_off,cast_off,throw,hurl,bedevil,thrust,befuddle</rdfs:comment>
        <rdfs:comment xml:lang="callstatement">throwAway</rdfs:comment>
        <rdfs:label xml:lang="en">throwAway</rdfs:label>
    </owl:NamedIndividual>
    


    <!-- Optional[http://www.semanticweb.org/team3/robo-ontology-0]/#time_379b6aea_733e_4f0a_9bbd_26ba641409c5 -->

    <owl:NamedIndividual rdf:about="Optional[http://www.semanticweb.org/team3/robo-ontology-0]/#time_379b6aea_733e_4f0a_9bbd_26ba641409c5">
        <rdf:type rdf:resource="http://www.semanticweb.org/team3/robo-ontology-0#Parameter"/>
        <ofDataType rdf:resource="Optional[http://www.semanticweb.org/team3/robo-ontology-0]/#long"/>
        <rdfs:comment xml:lang="pos">1</rdfs:comment>
        <rdfs:label xml:lang="en">time</rdfs:label>
    </owl:NamedIndividual>
    


    <!-- Optional[http://www.semanticweb.org/team3/robo-ontology-0]/#time_46b7b4f4_e3dd_424d_8d16_797b1c201f13 -->

    <owl:NamedIndividual rdf:about="Optional[http://www.semanticweb.org/team3/robo-ontology-0]/#time_46b7b4f4_e3dd_424d_8d16_797b1c201f13">
        <rdf:type rdf:resource="http://www.semanticweb.org/team3/robo-ontology-0#Parameter"/>
        <ofDataType rdf:resource="Optional[http://www.semanticweb.org/team3/robo-ontology-0]/#long"/>
        <rdfs:comment xml:lang="pos">1</rdfs:comment>
        <rdfs:label xml:lang="en">time</rdfs:label>
    </owl:NamedIndividual>
    


    <!-- Optional[http://www.semanticweb.org/team3/robo-ontology-0]/#turnAround_475a5059_24e9_4986_87c4_cab2e163406d -->

    <owl:NamedIndividual rdf:about="Optional[http://www.semanticweb.org/team3/robo-ontology-0]/#turnAround_475a5059_24e9_4986_87c4_cab2e163406d">
        <rdf:type rdf:resource="http://www.semanticweb.org/team3/robo-ontology-0#Method"/>
        <hasParameter rdf:resource="Optional[http://www.semanticweb.org/team3/robo-ontology-0]/#speed_380373bb_b428_4a6c_b553_779f56c0c983"/>
        <rdfs:comment xml:lang="synonym">Around:</rdfs:comment>
        <rdfs:comment xml:lang="importstatement">edu.kit.ipd.ev3.IRobo</rdfs:comment>
        <rdfs:comment xml:lang="synonym">turn: turn_over,grow,release,deform,work,plough,rick,turn,reverse,sour,sprain,change_state,wrench,change_by_reversal,plow,move_around,call_on,wrick,flex,bend,twist,become,ferment</rdfs:comment>
        <rdfs:comment xml:lang="callstatement">turnAround</rdfs:comment>
        <rdfs:label xml:lang="en">turnAround</rdfs:label>
    </owl:NamedIndividual>
    


    <!-- Optional[http://www.semanticweb.org/team3/robo-ontology-0]/#turnAround_77484764_3673_447c_8e89_2667fcd6185d -->

    <owl:NamedIndividual rdf:about="Optional[http://www.semanticweb.org/team3/robo-ontology-0]/#turnAround_77484764_3673_447c_8e89_2667fcd6185d">
        <rdf:type rdf:resource="http://www.semanticweb.org/team3/robo-ontology-0#Method"/>
        <rdfs:comment xml:lang="synonym">Around:</rdfs:comment>
        <rdfs:comment xml:lang="importstatement">edu.kit.ipd.ev3.IRobo</rdfs:comment>
        <rdfs:comment xml:lang="synonym">turn: turn_over,grow,release,deform,work,plough,rick,turn,reverse,sour,sprain,change_state,wrench,change_by_reversal,plow,move_around,call_on,wrick,flex,bend,twist,become,ferment</rdfs:comment>
        <rdfs:comment xml:lang="callstatement">turnAround</rdfs:comment>
        <rdfs:label xml:lang="en">turnAround</rdfs:label>
    </owl:NamedIndividual>
    


    <!-- Optional[http://www.semanticweb.org/team3/robo-ontology-0]/#turnUntil_1018bea4_defa_49eb_a1de_18d649ae62a8 -->

    <owl:NamedIndividual rdf:about="Optional[http://www.semanticweb.org/team3/robo-ontology-0]/#turnUntil_1018bea4_defa_49eb_a1de_18d649ae62a8">
        <rdf:type rdf:resource="http://www.semanticweb.org/team3/robo-ontology-0#Method"/>
        <hasParameter rdf:resource="Optional[http://www.semanticweb.org/team3/robo-ontology-0]/#condition_1fa277eb_6ad6_4375_b1bf_a235bc5c60d0"/>
        <hasParameter rdf:resource="Optional[http://www.semanticweb.org/team3/robo-ontology-0]/#dir_9b678577_ca1c_4506_bdd2_82f9c0e20595"/>
        <hasParameter rdf:resource="Optional[http://www.semanticweb.org/team3/robo-ontology-0]/#speed_89664740_d918_4358_b515_992fd86b6143"/>
        <rdfs:comment xml:lang="importstatement">edu.kit.ipd.ev3.IRobo</rdfs:comment>
        <rdfs:comment xml:lang="synonym">turn: turn_over,grow,release,deform,work,plough,rick,turn,reverse,sour,sprain,change_state,wrench,change_by_reversal,plow,move_around,call_on,wrick,flex,bend,twist,become,ferment</rdfs:comment>
        <rdfs:comment xml:lang="callstatement">turnUntil</rdfs:comment>
        <rdfs:label xml:lang="en">turnUntil</rdfs:label>
    </owl:NamedIndividual>
    


    <!-- Optional[http://www.semanticweb.org/team3/robo-ontology-0]/#turnUntil_146975b8_c2fc_4f4f_839d_68245ee2c486 -->

    <owl:NamedIndividual rdf:about="Optional[http://www.semanticweb.org/team3/robo-ontology-0]/#turnUntil_146975b8_c2fc_4f4f_839d_68245ee2c486">
        <rdf:type rdf:resource="http://www.semanticweb.org/team3/robo-ontology-0#Method"/>
        <hasParameter rdf:resource="Optional[http://www.semanticweb.org/team3/robo-ontology-0]/#condition_c9954084_3136_4c88_a6e5_13b0496b2642"/>
        <hasParameter rdf:resource="Optional[http://www.semanticweb.org/team3/robo-ontology-0]/#dir_c2408af1_cd85_4bce_bf9a_93015ed8bf5e"/>
        <rdfs:comment xml:lang="importstatement">edu.kit.ipd.ev3.IRobo</rdfs:comment>
        <rdfs:comment xml:lang="synonym">turn: turn_over,grow,release,deform,work,plough,rick,turn,reverse,sour,sprain,change_state,wrench,change_by_reversal,plow,move_around,call_on,wrick,flex,bend,twist,become,ferment</rdfs:comment>
        <rdfs:comment xml:lang="callstatement">turnUntil</rdfs:comment>
        <rdfs:label xml:lang="en">turnUntil</rdfs:label>
    </owl:NamedIndividual>
    


    <!-- Optional[http://www.semanticweb.org/team3/robo-ontology-0]/#turnUntil_e9665014_a791_47dc_bcea_4850025b356b -->

    <owl:NamedIndividual rdf:about="Optional[http://www.semanticweb.org/team3/robo-ontology-0]/#turnUntil_e9665014_a791_47dc_bcea_4850025b356b">
        <rdf:type rdf:resource="http://www.semanticweb.org/team3/robo-ontology-0#Method"/>
        <hasParameter rdf:resource="Optional[http://www.semanticweb.org/team3/robo-ontology-0]/#condition_236a119c_ede1_43c8_968f_9ce1f5d0fa43"/>
        <rdfs:comment xml:lang="importstatement">edu.kit.ipd.ev3.IRobo</rdfs:comment>
        <rdfs:comment xml:lang="synonym">turn: turn_over,grow,release,deform,work,plough,rick,turn,reverse,sour,sprain,change_state,wrench,change_by_reversal,plow,move_around,call_on,wrick,flex,bend,twist,become,ferment</rdfs:comment>
        <rdfs:comment xml:lang="callstatement">turnUntil</rdfs:comment>
        <rdfs:label xml:lang="en">turnUntil</rdfs:label>
    </owl:NamedIndividual>
    


    <!-- Optional[http://www.semanticweb.org/team3/robo-ontology-0]/#turnUntil_eec343ae_6826_45d4_b1e5_374ba890ff19 -->

    <owl:NamedIndividual rdf:about="Optional[http://www.semanticweb.org/team3/robo-ontology-0]/#turnUntil_eec343ae_6826_45d4_b1e5_374ba890ff19">
        <rdf:type rdf:resource="http://www.semanticweb.org/team3/robo-ontology-0#Method"/>
        <hasParameter rdf:resource="Optional[http://www.semanticweb.org/team3/robo-ontology-0]/#condition_f2c54d55_fac2_4c1f_a8c9_f7e225fd2f9a"/>
        <hasParameter rdf:resource="Optional[http://www.semanticweb.org/team3/robo-ontology-0]/#speed_5bff6444_195d_489a_8c6d_99d9aa8ae08b"/>
        <rdfs:comment xml:lang="importstatement">edu.kit.ipd.ev3.IRobo</rdfs:comment>
        <rdfs:comment xml:lang="synonym">turn: turn_over,grow,release,deform,work,plough,rick,turn,reverse,sour,sprain,change_state,wrench,change_by_reversal,plow,move_around,call_on,wrick,flex,bend,twist,become,ferment</rdfs:comment>
        <rdfs:comment xml:lang="callstatement">turnUntil</rdfs:comment>
        <rdfs:label xml:lang="en">turnUntil</rdfs:label>
    </owl:NamedIndividual>
    


    <!-- Optional[http://www.semanticweb.org/team3/robo-ontology-0]/#turn_015380b0_1956_4823_af4c_0f1ca74b18a0 -->

    <owl:NamedIndividual rdf:about="Optional[http://www.semanticweb.org/team3/robo-ontology-0]/#turn_015380b0_1956_4823_af4c_0f1ca74b18a0">
        <rdf:type rdf:resource="http://www.semanticweb.org/team3/robo-ontology-0#Method"/>
        <hasParameter rdf:resource="Optional[http://www.semanticweb.org/team3/robo-ontology-0]/#rev_4c1bc855_4541_46de_af2a_163088812227"/>
        <hasParameter rdf:resource="Optional[http://www.semanticweb.org/team3/robo-ontology-0]/#speed_920277e4_7341_4e21_a0b8_84150fa97224"/>
        <rdfs:comment xml:lang="importstatement">edu.kit.ipd.ev3.IRobo</rdfs:comment>
        <rdfs:comment xml:lang="callstatement">turn</rdfs:comment>
        <rdfs:comment xml:lang="synonym">turn: turn_over,grow,release,deform,work,plough,rick,turn,reverse,sour,sprain,change_state,wrench,change_by_reversal,plow,move_around,call_on,wrick,flex,bend,twist,become,ferment</rdfs:comment>
        <rdfs:label xml:lang="en">turn</rdfs:label>
    </owl:NamedIndividual>
    


    <!-- Optional[http://www.semanticweb.org/team3/robo-ontology-0]/#turn_15018856_e385_4daf_8ac7_f15a3a988e6f -->

    <owl:NamedIndividual rdf:about="Optional[http://www.semanticweb.org/team3/robo-ontology-0]/#turn_15018856_e385_4daf_8ac7_f15a3a988e6f">
        <rdf:type rdf:resource="http://www.semanticweb.org/team3/robo-ontology-0#Method"/>
        <hasParameter rdf:resource="Optional[http://www.semanticweb.org/team3/robo-ontology-0]/#dir_456efe65_c422_4fd1_804d_82a2f74ef433"/>
        <rdfs:comment xml:lang="importstatement">edu.kit.ipd.ev3.IRobo</rdfs:comment>
        <rdfs:comment xml:lang="callstatement">turn</rdfs:comment>
        <rdfs:comment xml:lang="synonym">turn: turn_over,grow,release,deform,work,plough,rick,turn,reverse,sour,sprain,change_state,wrench,change_by_reversal,plow,move_around,call_on,wrick,flex,bend,twist,become,ferment</rdfs:comment>
        <rdfs:label xml:lang="en">turn</rdfs:label>
    </owl:NamedIndividual>
    


    <!-- Optional[http://www.semanticweb.org/team3/robo-ontology-0]/#turn_20324a8e_5582_49c2_8207_2f4b7b3325e4 -->

    <owl:NamedIndividual rdf:about="Optional[http://www.semanticweb.org/team3/robo-ontology-0]/#turn_20324a8e_5582_49c2_8207_2f4b7b3325e4">
        <rdf:type rdf:resource="http://www.semanticweb.org/team3/robo-ontology-0#Method"/>
        <hasParameter rdf:resource="Optional[http://www.semanticweb.org/team3/robo-ontology-0]/#degrees_1d01bf9a_b37b_4e6b_9269_02a14a71a377"/>
        <hasParameter rdf:resource="Optional[http://www.semanticweb.org/team3/robo-ontology-0]/#dir_6c6821d0_0b6f_4abd_84a8_51d5562bebdd"/>
        <hasParameter rdf:resource="Optional[http://www.semanticweb.org/team3/robo-ontology-0]/#speed_ecaafbbb_46d9_4303_968a_a64bc1029fab"/>
        <rdfs:comment xml:lang="importstatement">edu.kit.ipd.ev3.IRobo</rdfs:comment>
        <rdfs:comment xml:lang="callstatement">turn</rdfs:comment>
        <rdfs:comment xml:lang="synonym">turn: turn_over,grow,release,deform,work,plough,rick,turn,reverse,sour,sprain,change_state,wrench,change_by_reversal,plow,move_around,call_on,wrick,flex,bend,twist,become,ferment</rdfs:comment>
        <rdfs:label xml:lang="en">turn</rdfs:label>
    </owl:NamedIndividual>
    


    <!-- Optional[http://www.semanticweb.org/team3/robo-ontology-0]/#turn_429073be_002d_4670_92d1_a59f7186079e -->

    <owl:NamedIndividual rdf:about="Optional[http://www.semanticweb.org/team3/robo-ontology-0]/#turn_429073be_002d_4670_92d1_a59f7186079e">
        <rdf:type rdf:resource="http://www.semanticweb.org/team3/robo-ontology-0#Method"/>
        <hasParameter rdf:resource="Optional[http://www.semanticweb.org/team3/robo-ontology-0]/#degrees_86efca15_f77e_4e27_8f39_667885e65e6b"/>
        <rdfs:comment xml:lang="importstatement">edu.kit.ipd.ev3.IRobo</rdfs:comment>
        <rdfs:comment xml:lang="callstatement">turn</rdfs:comment>
        <rdfs:comment xml:lang="synonym">turn: turn_over,grow,release,deform,work,plough,rick,turn,reverse,sour,sprain,change_state,wrench,change_by_reversal,plow,move_around,call_on,wrick,flex,bend,twist,become,ferment</rdfs:comment>
        <rdfs:label xml:lang="en">turn</rdfs:label>
    </owl:NamedIndividual>
    


    <!-- Optional[http://www.semanticweb.org/team3/robo-ontology-0]/#turn_907fee24_acb5_479f_9605_2c7047858c97 -->

    <owl:NamedIndividual rdf:about="Optional[http://www.semanticweb.org/team3/robo-ontology-0]/#turn_907fee24_acb5_479f_9605_2c7047858c97">
        <rdf:type rdf:resource="http://www.semanticweb.org/team3/robo-ontology-0#Method"/>
        <hasParameter rdf:resource="Optional[http://www.semanticweb.org/team3/robo-ontology-0]/#rev_8f4d3bfc_5595_4ba3_8863_8e88ea42a574"/>
        <rdfs:comment xml:lang="importstatement">edu.kit.ipd.ev3.IRobo</rdfs:comment>
        <rdfs:comment xml:lang="callstatement">turn</rdfs:comment>
        <rdfs:comment xml:lang="synonym">turn: turn_over,grow,release,deform,work,plough,rick,turn,reverse,sour,sprain,change_state,wrench,change_by_reversal,plow,move_around,call_on,wrick,flex,bend,twist,become,ferment</rdfs:comment>
        <rdfs:label xml:lang="en">turn</rdfs:label>
    </owl:NamedIndividual>
    


    <!-- Optional[http://www.semanticweb.org/team3/robo-ontology-0]/#turn_bb60505a_f514_41cc_8246_e299c9060aa6 -->

    <owl:NamedIndividual rdf:about="Optional[http://www.semanticweb.org/team3/robo-ontology-0]/#turn_bb60505a_f514_41cc_8246_e299c9060aa6">
        <rdf:type rdf:resource="http://www.semanticweb.org/team3/robo-ontology-0#Method"/>
        <hasParameter rdf:resource="Optional[http://www.semanticweb.org/team3/robo-ontology-0]/#dir_4d27670d_4910_4c3e_99f7_c6b76468ebbd"/>
        <hasParameter rdf:resource="Optional[http://www.semanticweb.org/team3/robo-ontology-0]/#rev_24a66090_a410_4a79_a000_07f20e71b05f"/>
        <rdfs:comment xml:lang="importstatement">edu.kit.ipd.ev3.IRobo</rdfs:comment>
        <rdfs:comment xml:lang="callstatement">turn</rdfs:comment>
        <rdfs:comment xml:lang="synonym">turn: turn_over,grow,release,deform,work,plough,rick,turn,reverse,sour,sprain,change_state,wrench,change_by_reversal,plow,move_around,call_on,wrick,flex,bend,twist,become,ferment</rdfs:comment>
        <rdfs:label xml:lang="en">turn</rdfs:label>
    </owl:NamedIndividual>
    


    <!-- Optional[http://www.semanticweb.org/team3/robo-ontology-0]/#turn_c551826f_033a_4c38_a61d_15a09c497816 -->

    <owl:NamedIndividual rdf:about="Optional[http://www.semanticweb.org/team3/robo-ontology-0]/#turn_c551826f_033a_4c38_a61d_15a09c497816">
        <rdf:type rdf:resource="http://www.semanticweb.org/team3/robo-ontology-0#Method"/>
        <hasParameter rdf:resource="Optional[http://www.semanticweb.org/team3/robo-ontology-0]/#dir_abb1381b_479c_4ce3_a599_6cb3441ebf89"/>
        <hasParameter rdf:resource="Optional[http://www.semanticweb.org/team3/robo-ontology-0]/#rev_8700ae64_ffb9_45ed_8d20_0f865c4a96c0"/>
        <hasParameter rdf:resource="Optional[http://www.semanticweb.org/team3/robo-ontology-0]/#speed_3163d405_0aae_4b21_99ff_11acf5012130"/>
        <rdfs:comment xml:lang="importstatement">edu.kit.ipd.ev3.IRobo</rdfs:comment>
        <rdfs:comment xml:lang="callstatement">turn</rdfs:comment>
        <rdfs:comment xml:lang="synonym">turn: turn_over,grow,release,deform,work,plough,rick,turn,reverse,sour,sprain,change_state,wrench,change_by_reversal,plow,move_around,call_on,wrick,flex,bend,twist,become,ferment</rdfs:comment>
        <rdfs:label xml:lang="en">turn</rdfs:label>
    </owl:NamedIndividual>
    


    <!-- Optional[http://www.semanticweb.org/team3/robo-ontology-0]/#turn_d89c8822_ca9b_45b9_9336_d6c9331f06d5 -->

    <owl:NamedIndividual rdf:about="Optional[http://www.semanticweb.org/team3/robo-ontology-0]/#turn_d89c8822_ca9b_45b9_9336_d6c9331f06d5">
        <rdf:type rdf:resource="http://www.semanticweb.org/team3/robo-ontology-0#Method"/>
        <hasParameter rdf:resource="Optional[http://www.semanticweb.org/team3/robo-ontology-0]/#dir_5ec1806c_1162_4df5_b998_7d0f64c07c18"/>
        <hasParameter rdf:resource="Optional[http://www.semanticweb.org/team3/robo-ontology-0]/#speed_839c7b48_927a_4a06_bbd3_24a364489f5b"/>
        <rdfs:comment xml:lang="importstatement">edu.kit.ipd.ev3.IRobo</rdfs:comment>
        <rdfs:comment xml:lang="callstatement">turn</rdfs:comment>
        <rdfs:comment xml:lang="synonym">turn: turn_over,grow,release,deform,work,plough,rick,turn,reverse,sour,sprain,change_state,wrench,change_by_reversal,plow,move_around,call_on,wrick,flex,bend,twist,become,ferment</rdfs:comment>
        <rdfs:label xml:lang="en">turn</rdfs:label>
    </owl:NamedIndividual>
    


    <!-- Optional[http://www.semanticweb.org/team3/robo-ontology-0]/#turn_eaaa623e_708d_442e_acc8_289e522c6c09 -->

    <owl:NamedIndividual rdf:about="Optional[http://www.semanticweb.org/team3/robo-ontology-0]/#turn_eaaa623e_708d_442e_acc8_289e522c6c09">
        <rdf:type rdf:resource="http://www.semanticweb.org/team3/robo-ontology-0#Method"/>
        <hasParameter rdf:resource="Optional[http://www.semanticweb.org/team3/robo-ontology-0]/#degrees_bcac42d9_845b_48b8_bb49_703c21041c26"/>
        <hasParameter rdf:resource="Optional[http://www.semanticweb.org/team3/robo-ontology-0]/#speed_f476e627_864c_41e2_9f24_deb1e70bd7d6"/>
        <rdfs:comment xml:lang="importstatement">edu.kit.ipd.ev3.IRobo</rdfs:comment>
        <rdfs:comment xml:lang="callstatement">turn</rdfs:comment>
        <rdfs:comment xml:lang="synonym">turn: turn_over,grow,release,deform,work,plough,rick,turn,reverse,sour,sprain,change_state,wrench,change_by_reversal,plow,move_around,call_on,wrick,flex,bend,twist,become,ferment</rdfs:comment>
        <rdfs:label xml:lang="en">turn</rdfs:label>
    </owl:NamedIndividual>
    


    <!-- Optional[http://www.semanticweb.org/team3/robo-ontology-0]/#turn_f6f73b8b_a875_4174_9790_6253db4c54fb -->

    <owl:NamedIndividual rdf:about="Optional[http://www.semanticweb.org/team3/robo-ontology-0]/#turn_f6f73b8b_a875_4174_9790_6253db4c54fb">
        <rdf:type rdf:resource="http://www.semanticweb.org/team3/robo-ontology-0#Method"/>
        <hasParameter rdf:resource="Optional[http://www.semanticweb.org/team3/robo-ontology-0]/#degrees_97cd9f0f_1f53_4edd_b95e_f3888dfdcc25"/>
        <hasParameter rdf:resource="Optional[http://www.semanticweb.org/team3/robo-ontology-0]/#dir_105a0f66_e5d0_47dd_b6b4_e88b4dcaf3a5"/>
        <rdfs:comment xml:lang="importstatement">edu.kit.ipd.ev3.IRobo</rdfs:comment>
        <rdfs:comment xml:lang="callstatement">turn</rdfs:comment>
        <rdfs:comment xml:lang="synonym">turn: turn_over,grow,release,deform,work,plough,rick,turn,reverse,sour,sprain,change_state,wrench,change_by_reversal,plow,move_around,call_on,wrick,flex,bend,twist,become,ferment</rdfs:comment>
        <rdfs:label xml:lang="en">turn</rdfs:label>
    </owl:NamedIndividual>
    


    <!-- Optional[http://www.semanticweb.org/team3/robo-ontology-0]/#up -->

    <owl:NamedIndividual rdf:about="Optional[http://www.semanticweb.org/team3/robo-ontology-0]/#up">
        <rdf:type rdf:resource="http://www.semanticweb.org/team3/robo-ontology-0#Value"/>
        <rdfs:comment xml:lang="callstatement">UP</rdfs:comment>
        <rdfs:comment xml:lang="importstatement">edu.kit.ipd.ev3.enums.Direction</rdfs:comment>
        <rdfs:comment xml:lang="synonym">up: improving,astir,up,upward</rdfs:comment>
    </owl:NamedIndividual>
    


    <!-- Optional[http://www.semanticweb.org/team3/robo-ontology-0]/#white -->

    <owl:NamedIndividual rdf:about="Optional[http://www.semanticweb.org/team3/robo-ontology-0]/#white">
        <rdf:type rdf:resource="http://www.semanticweb.org/team3/robo-ontology-0#Value"/>
        <rdfs:comment xml:lang="callstatement">WHITE</rdfs:comment>
        <rdfs:comment xml:lang="importstatement">edu.kit.ipd.ev3.enums.Color</rdfs:comment>
        <rdfs:comment xml:lang="synonym">white: lily-white,bloodless,blank,ashen,white,white-hot,whitened,livid,clean,blanched,snowy</rdfs:comment>
    </owl:NamedIndividual>
    


    <!-- Optional[http://www.semanticweb.org/team3/robo-ontology-0]/#yellow -->

    <owl:NamedIndividual rdf:about="Optional[http://www.semanticweb.org/team3/robo-ontology-0]/#yellow">
        <rdf:type rdf:resource="http://www.semanticweb.org/team3/robo-ontology-0#Value"/>
        <rdfs:comment xml:lang="callstatement">YELLOW</rdfs:comment>
        <rdfs:comment xml:lang="importstatement">edu.kit.ipd.ev3.enums.Color</rdfs:comment>
        <rdfs:comment xml:lang="synonym">yellow: chicken,yellowish,jaundiced,xanthous,lily-livered,yellowed,yellow,icteric,scandalmongering,sensationalistic,white-livered,yellow-bellied,chickenhearted</rdfs:comment>
    </owl:NamedIndividual>
    


    <!-- http://www.semanticweb.org/team3/robo-ontology-0#OWLNamedIndividual_1bcc52ff_106d_4230_9109_17959e82c023 -->

    <owl:NamedIndividual rdf:about="http://www.semanticweb.org/team3/robo-ontology-0#OWLNamedIndividual_1bcc52ff_106d_4230_9109_17959e82c023">
        <rdf:type rdf:resource="http://www.semanticweb.org/team3/robo-ontology-0#Object"/>
        <closeDistance rdf:datatype="http://www.w3.org/2001/XMLSchema#double">32.0</closeDistance>
        <farDistance rdf:datatype="http://www.w3.org/2001/XMLSchema#double">65.0</farDistance>
        <midDistance rdf:datatype="http://www.w3.org/2001/XMLSchema#double">41.0</midDistance>
        <rdfs:comment xml:lang="synonym">Cleaner: dry_cleaner,cleaner,cleansing_agent,cleanser</rdfs:comment>
        <rdfs:comment xml:lang="synonym">Screen: cover,blind,filmdom,silver_screen,concealment,screen,projection_screen,CRT_screen,sieve,screenland,covert</rdfs:comment>
        <rdfs:label xml:lang="en">ScreenCleaner</rdfs:label>
    </owl:NamedIndividual>
    


    <!-- http://www.semanticweb.org/team3/robo-ontology-0#OWLNamedIndividual_3d853fb8_7c74_47bd_837e_26a1c791b778 -->

    <owl:NamedIndividual rdf:about="http://www.semanticweb.org/team3/robo-ontology-0#OWLNamedIndividual_3d853fb8_7c74_47bd_837e_26a1c791b778">
        <rdf:type rdf:resource="http://www.semanticweb.org/team3/robo-ontology-0#Object"/>
        <closeDistance rdf:datatype="http://www.w3.org/2001/XMLSchema#double">88.0</closeDistance>
        <farDistance rdf:datatype="http://www.w3.org/2001/XMLSchema#double">70.0</farDistance>
        <midDistance rdf:datatype="http://www.w3.org/2001/XMLSchema#double">42.0</midDistance>
        <rdfs:comment xml:lang="synonym">Daemmstoff:</rdfs:comment>
        <rdfs:label xml:lang="en">Daemmstoff</rdfs:label>
    </owl:NamedIndividual>
    


    <!-- http://www.semanticweb.org/team3/robo-ontology-0#OWLNamedIndividual_3e484dd5_5492_44c2_ae49_bcde650f1a0e -->

    <owl:NamedIndividual rdf:about="http://www.semanticweb.org/team3/robo-ontology-0#OWLNamedIndividual_3e484dd5_5492_44c2_ae49_bcde650f1a0e">
        <rdf:type rdf:resource="http://www.semanticweb.org/team3/robo-ontology-0#Object"/>
        <closeDistance rdf:datatype="http://www.w3.org/2001/XMLSchema#double">25.0</closeDistance>
        <farDistance rdf:datatype="http://www.w3.org/2001/XMLSchema#double">66.0</farDistance>
        <midDistance rdf:datatype="http://www.w3.org/2001/XMLSchema#double">35.0</midDistance>
        <rdfs:comment xml:lang="synonym">Box: loge,corner,box_seat,boxwood,box,boxful</rdfs:comment>
        <rdfs:comment xml:lang="synonym">Tea: tea,teatime,afternoon_tea,tea_leaf,Camellia_sinensis</rdfs:comment>
        <rdfs:label xml:lang="en">TeaBox</rdfs:label>
    </owl:NamedIndividual>
    


    <!-- http://www.semanticweb.org/team3/robo-ontology-0#OWLNamedIndividual_60884d29_7b1d_4765_8b59_96be4b6fc128 -->

    <owl:NamedIndividual rdf:about="http://www.semanticweb.org/team3/robo-ontology-0#OWLNamedIndividual_60884d29_7b1d_4765_8b59_96be4b6fc128">
        <rdf:type rdf:resource="http://www.semanticweb.org/team3/robo-ontology-0#Object"/>
        <closeDistance rdf:datatype="http://www.w3.org/2001/XMLSchema#double">9.5</closeDistance>
        <farDistance rdf:datatype="http://www.w3.org/2001/XMLSchema#double">70.0</farDistance>
        <midDistance rdf:datatype="http://www.w3.org/2001/XMLSchema#double">41.0</midDistance>
        <rdfs:comment xml:lang="synonym">Beer: beer</rdfs:comment>
        <rdfs:comment xml:lang="synonym">Black: black-market,ignominious,smuggled,fateful,contraband,bootleg,calamitous,pitch-dark,black,disgraceful,opprobrious,dim,smutty,fatal,bleak,inglorious,disastrous,mordant,blackened,sinister,dark,shameful,pitch-black,grim</rdfs:comment>
        <rdfs:comment xml:lang="synonym">Can: ass,prat,behind,stool,commode,potty,lavatory,backside,throne,tooshie,keister,tin_can,can,rear,fundament,rump,rear_end,pot,fanny,canful,tin,hind_end,derriere,hindquarters,bathroom,tush,lav,can_buoy,crapper,tail,bottom,posterior,stern,arse,seat,toilet,nates,privy,buns,buttocks,john,bum,tail_end,butt</rdfs:comment>
        <rdfs:label xml:lang="en">BlackBeerCan</rdfs:label>
    </owl:NamedIndividual>
    


    <!-- http://www.semanticweb.org/team3/robo-ontology-0#OWLNamedIndividual_92801afe_9bc4_4b60_8b2d_8e923fc5e064 -->

    <owl:NamedIndividual rdf:about="http://www.semanticweb.org/team3/robo-ontology-0#OWLNamedIndividual_92801afe_9bc4_4b60_8b2d_8e923fc5e064">
        <rdf:type rdf:resource="http://www.semanticweb.org/team3/robo-ontology-0#Object"/>
        <closeDistance rdf:datatype="http://www.w3.org/2001/XMLSchema#double">6.0</closeDistance>
        <farDistance rdf:datatype="http://www.w3.org/2001/XMLSchema#double">72.0</farDistance>
        <midDistance rdf:datatype="http://www.w3.org/2001/XMLSchema#double">40.0</midDistance>
        <rdfs:comment xml:lang="synonym">Bottle: feeding_bottle,bottle,bottleful,nursing_bottle</rdfs:comment>
        <rdfs:comment xml:lang="synonym">Cup: loving_cup,cupful,cup</rdfs:comment>
        <rdfs:comment xml:lang="synonym">Suction: sucking,suction,suck</rdfs:comment>
        <rdfs:label xml:lang="en">SuctionCupBottle</rdfs:label>
    </owl:NamedIndividual>
    


    <!-- http://www.semanticweb.org/team3/robo-ontology-0#OWLNamedIndividual_94ae6160_e029_4e08_87f4_672e319fc7eb -->

    <owl:NamedIndividual rdf:about="http://www.semanticweb.org/team3/robo-ontology-0#OWLNamedIndividual_94ae6160_e029_4e08_87f4_672e319fc7eb">
        <rdf:type rdf:resource="http://www.semanticweb.org/team3/robo-ontology-0#Object"/>
        <closeDistance rdf:datatype="http://www.w3.org/2001/XMLSchema#double">12.7</closeDistance>
        <farDistance rdf:datatype="http://www.w3.org/2001/XMLSchema#double">55.0</farDistance>
        <midDistance rdf:datatype="http://www.w3.org/2001/XMLSchema#double">39.0</midDistance>
        <rdfs:comment xml:lang="synonym">Nuts:</rdfs:comment>
        <rdfs:label xml:lang="en">Nuts</rdfs:label>
    </owl:NamedIndividual>
    


    <!-- http://www.semanticweb.org/team3/robo-ontology-0#OWLNamedIndividual_9f1154b7_a545_485f_8866_4b1394e98191 -->

    <owl:NamedIndividual rdf:about="http://www.semanticweb.org/team3/robo-ontology-0#OWLNamedIndividual_9f1154b7_a545_485f_8866_4b1394e98191">
        <rdf:type rdf:resource="http://www.semanticweb.org/team3/robo-ontology-0#Object"/>
        <closeDistance rdf:datatype="http://www.w3.org/2001/XMLSchema#double">10.0</closeDistance>
        <farDistance rdf:datatype="http://www.w3.org/2001/XMLSchema#double">71.0</farDistance>
        <midDistance rdf:datatype="http://www.w3.org/2001/XMLSchema#double">40.0</midDistance>
        <rdfs:comment xml:lang="synonym">Beer: beer</rdfs:comment>
        <rdfs:comment xml:lang="synonym">Can: ass,prat,behind,stool,commode,potty,lavatory,backside,throne,tooshie,keister,tin_can,can,rear,fundament,rump,rear_end,pot,fanny,canful,tin,hind_end,derriere,hindquarters,bathroom,tush,lav,can_buoy,crapper,tail,bottom,posterior,stern,arse,seat,toilet,nates,privy,buns,buttocks,john,bum,tail_end,butt</rdfs:comment>
        <rdfs:comment xml:lang="synonym">Red: cherry,violent,cherry-red,ruby-red,ruddy,reddened,flushed,carmine,ruby,red,scarlet,crimson,blood-red,reddish,cerise,red-faced</rdfs:comment>
        <rdfs:label xml:lang="en">RedBeerCan</rdfs:label>
    </owl:NamedIndividual>
    


    <!-- http://www.semanticweb.org/team3/robo-ontology-0#OWLNamedIndividual_bf3213cc_7d10_49d5_bffe_cf4e601d427b -->

    <owl:NamedIndividual rdf:about="http://www.semanticweb.org/team3/robo-ontology-0#OWLNamedIndividual_bf3213cc_7d10_49d5_bffe_cf4e601d427b">
        <rdf:type rdf:resource="http://www.semanticweb.org/team3/robo-ontology-0#Object"/>
        <closeDistance rdf:datatype="http://www.w3.org/2001/XMLSchema#double">255.0</closeDistance>
        <farDistance rdf:datatype="http://www.w3.org/2001/XMLSchema#double">77.0</farDistance>
        <midDistance rdf:datatype="http://www.w3.org/2001/XMLSchema#double">40.0</midDistance>
        <rdfs:comment xml:lang="synonym">Ball: Ball,egg,Lucille_Ball,glob,baseball_game,chunk,clump,testis,testicle,orchis,nut,clod,formal,ball,musket_ball,globe,ballock,baseball,bollock,orb,lump</rdfs:comment>
        <rdfs:comment xml:lang="synonym">Gum: mucilage,gingiva,chewing_gum,glue,gumwood,gum_tree,gum</rdfs:comment>
        <rdfs:comment xml:lang="synonym">spiky: peaky,spiky</rdfs:comment>
        <rdfs:label xml:lang="en">spikyGumBall</rdfs:label>
    </owl:NamedIndividual>
    


    <!-- http://www.semanticweb.org/team3/robo-ontology-0#OWLNamedIndividual_e22de7be_9327_4c16_987c_0e3f6ae516a0 -->

    <owl:NamedIndividual rdf:about="http://www.semanticweb.org/team3/robo-ontology-0#OWLNamedIndividual_e22de7be_9327_4c16_987c_0e3f6ae516a0">
        <rdf:type rdf:resource="http://www.semanticweb.org/team3/robo-ontology-0#Object"/>
        <closeDistance rdf:datatype="http://www.w3.org/2001/XMLSchema#double">25.0</closeDistance>
        <farDistance rdf:datatype="http://www.w3.org/2001/XMLSchema#double">72.0</farDistance>
        <midDistance rdf:datatype="http://www.w3.org/2001/XMLSchema#double">14.0</midDistance>
        <rdfs:comment xml:lang="synonym">Cup: loving_cup,cupful,cup</rdfs:comment>
        <rdfs:comment xml:lang="synonym">Xmas: Christmas,Dec_25,Christmas_Day,Xmas</rdfs:comment>
        <rdfs:label xml:lang="en">XmasCup</rdfs:label>
    </owl:NamedIndividual>
    


    <!-- http://www.semanticweb.org/team3/robo-ontology-0#OWLNamedIndividual_e22de7be_9327_4c16_987c_0e3f6ae542a0 -->

    <owl:NamedIndividual rdf:about="http://www.semanticweb.org/team3/robo-ontology-0#OWLNamedIndividual_e22de7be_9327_4c16_987c_0e3f6ae542a0">
        <rdf:type rdf:resource="http://www.semanticweb.org/team3/robo-ontology-0#Object"/>
        <closeDistance rdf:datatype="http://www.w3.org/2001/XMLSchema#double">32.0</closeDistance>
        <farDistance rdf:datatype="http://www.w3.org/2001/XMLSchema#double">70.0</farDistance>
        <midDistance rdf:datatype="http://www.w3.org/2001/XMLSchema#double">40.0</midDistance>
        <rdfs:comment xml:lang="synonym">Tissue: tissue_paper,tissue</rdfs:comment>
        <rdfs:label xml:lang="en">Tissue</rdfs:label>
    </owl:NamedIndividual>
    


    <!-- http://www.semanticweb.org/team3/robo-ontology-0#Object -->

    <owl:NamedIndividual rdf:about="http://www.semanticweb.org/team3/robo-ontology-0#Object">
        <rdf:type rdf:resource="http://www.semanticweb.org/team3/robo-ontology-0#DataType"/>
    </owl:NamedIndividual>
    


    <!-- http://www.semanticweb.org/team3/robo-ontology-0#Robo -->

    <owl:NamedIndividual rdf:about="http://www.semanticweb.org/team3/robo-ontology-0#Robo">
        <hasMethod rdf:resource="Optional[http://www.semanticweb.org/team3/robo-ontology-0]/#ConditionCloseToObject_06ee274d_73d9_44b1_96a5_24f057423e55"/>
        <hasMethod rdf:resource="Optional[http://www.semanticweb.org/team3/robo-ontology-0]/#ConditionLineDetected_e61c6675_10b2_4088_a3dd_14eadb032abf"/>
        <hasMethod rdf:resource="Optional[http://www.semanticweb.org/team3/robo-ontology-0]/#ConditionNearObject_2885ebd1_5cfe_415c_bef6_ed1585d260e0"/>
        <hasMethod rdf:resource="Optional[http://www.semanticweb.org/team3/robo-ontology-0]/#ConditionSeesColor_cd5a4bb8_73ff_4856_8f34_4d344853faef"/>
        <hasMethod rdf:resource="Optional[http://www.semanticweb.org/team3/robo-ontology-0]/#ConditionSeesObject_7e9019ee_89e0_4074_a791_7c746017f48a"/>
        <hasMethod rdf:resource="Optional[http://www.semanticweb.org/team3/robo-ontology-0]/#ConditionSeesRemote_e58532d7_fab9_464b_b33d_fe01e5ea353c"/>
        <hasMethod rdf:resource="Optional[http://www.semanticweb.org/team3/robo-ontology-0]/#belch_28769a70_ee6a_47dd_b208_a1f25667fb98"/>
        <hasMethod rdf:resource="Optional[http://www.semanticweb.org/team3/robo-ontology-0]/#blink_dba4b811_30ab_4865_b498_fc3c1c1c6c55"/>
        <hasMethod rdf:resource="Optional[http://www.semanticweb.org/team3/robo-ontology-0]/#clap_1aa775d3_be0f_492e_88ab_d5bf99aaf8a1"/>
        <hasMethod rdf:resource="Optional[http://www.semanticweb.org/team3/robo-ontology-0]/#followLineUntil_47c773f2_f939_41b7_a770_2f4a90b49e2e"/>
        <hasMethod rdf:resource="Optional[http://www.semanticweb.org/team3/robo-ontology-0]/#followLineUntil_b1141948_f721_4f2f_ab17_db74fbc5fb10"/>
        <hasMethod rdf:resource="Optional[http://www.semanticweb.org/team3/robo-ontology-0]/#grab_1d868109_1049_4bad_b334_f9289541520b"/>
        <hasMethod rdf:resource="Optional[http://www.semanticweb.org/team3/robo-ontology-0]/#liftHead_b56fe84f_82c1_4441_aecb_7c8624cff340"/>
        <hasMethod rdf:resource="Optional[http://www.semanticweb.org/team3/robo-ontology-0]/#look_6dbb4241_e4ae_4224_8a49_788d52a33877"/>
        <hasMethod rdf:resource="Optional[http://www.semanticweb.org/team3/robo-ontology-0]/#lowerHead_8d10f90b_e0aa_4647_87a3_5ff910ed72f3"/>
        <hasMethod rdf:resource="Optional[http://www.semanticweb.org/team3/robo-ontology-0]/#makeTowardsObject_408abcce_baac_479e_aa3f_d1ddbdc039ca"/>
        <hasMethod rdf:resource="Optional[http://www.semanticweb.org/team3/robo-ontology-0]/#moveHead_066f8b00_afb5_4294_932e_7d2b6affeee1"/>
        <hasMethod rdf:resource="Optional[http://www.semanticweb.org/team3/robo-ontology-0]/#moveUntil_cc47bc97_a95a_4277_83a7_1302c927988e"/>
        <hasMethod rdf:resource="Optional[http://www.semanticweb.org/team3/robo-ontology-0]/#moveUntil_ff3749ee_8ffb_4dd6_bb74_9a9f570def7c"/>
        <hasMethod rdf:resource="Optional[http://www.semanticweb.org/team3/robo-ontology-0]/#move_1b2b5e11_c82c_4937_8850_c3d59e2c1c15"/>
        <hasMethod rdf:resource="Optional[http://www.semanticweb.org/team3/robo-ontology-0]/#move_7815995a_f151_4e53_acd7_3770ade9e721"/>
        <hasMethod rdf:resource="Optional[http://www.semanticweb.org/team3/robo-ontology-0]/#move_a0eb6a93_ee54_4680_8963_d6249cb69791"/>
        <hasMethod rdf:resource="Optional[http://www.semanticweb.org/team3/robo-ontology-0]/#move_f06a062a_952c_4f07_9752_69c55b0140be"/>
        <hasMethod rdf:resource="Optional[http://www.semanticweb.org/team3/robo-ontology-0]/#move_fdd5345b_7ce2_4000_a81b_99529d0fd6db"/>
        <hasMethod rdf:resource="Optional[http://www.semanticweb.org/team3/robo-ontology-0]/#playHalloweenTheme_03b52809_060c_4641_bad6_7583e56ad53e"/>
        <hasMethod rdf:resource="Optional[http://www.semanticweb.org/team3/robo-ontology-0]/#release_23fd61bc_a93a_4590_b9af_c46197f9fdc9"/>
        <hasMethod rdf:resource="Optional[http://www.semanticweb.org/team3/robo-ontology-0]/#sayGoodbye_29e06e21_df38_4ac0_8b26_fe3580981233"/>
        <hasMethod rdf:resource="Optional[http://www.semanticweb.org/team3/robo-ontology-0]/#sing_e7266fd2_7104_4bc6_b8ba_595c3c4882a9"/>
        <hasMethod rdf:resource="Optional[http://www.semanticweb.org/team3/robo-ontology-0]/#throwAway_e5d7fcb6_3209_41a4_b516_4e356c46d717"/>
        <hasMethod rdf:resource="Optional[http://www.semanticweb.org/team3/robo-ontology-0]/#turnAround_475a5059_24e9_4986_87c4_cab2e163406d"/>
        <hasMethod rdf:resource="Optional[http://www.semanticweb.org/team3/robo-ontology-0]/#turnAround_77484764_3673_447c_8e89_2667fcd6185d"/>
        <hasMethod rdf:resource="Optional[http://www.semanticweb.org/team3/robo-ontology-0]/#turnUntil_1018bea4_defa_49eb_a1de_18d649ae62a8"/>
        <hasMethod rdf:resource="Optional[http://www.semanticweb.org/team3/robo-ontology-0]/#turnUntil_146975b8_c2fc_4f4f_839d_68245ee2c486"/>
        <hasMethod rdf:resource="Optional[http://www.semanticweb.org/team3/robo-ontology-0]/#turnUntil_e9665014_a791_47dc_bcea_4850025b356b"/>
        <hasMethod rdf:resource="Optional[http://www.semanticweb.org/team3/robo-ontology-0]/#turnUntil_eec343ae_6826_45d4_b1e5_374ba890ff19"/>
        <hasMethod rdf:resource="Optional[http://www.semanticweb.org/team3/robo-ontology-0]/#turn_015380b0_1956_4823_af4c_0f1ca74b18a0"/>
        <hasMethod rdf:resource="Optional[http://www.semanticweb.org/team3/robo-ontology-0]/#turn_15018856_e385_4daf_8ac7_f15a3a988e6f"/>
        <hasMethod rdf:resource="Optional[http://www.semanticweb.org/team3/robo-ontology-0]/#turn_20324a8e_5582_49c2_8207_2f4b7b3325e4"/>
        <hasMethod rdf:resource="Optional[http://www.semanticweb.org/team3/robo-ontology-0]/#turn_429073be_002d_4670_92d1_a59f7186079e"/>
        <hasMethod rdf:resource="Optional[http://www.semanticweb.org/team3/robo-ontology-0]/#turn_907fee24_acb5_479f_9605_2c7047858c97"/>
        <hasMethod rdf:resource="Optional[http://www.semanticweb.org/team3/robo-ontology-0]/#turn_bb60505a_f514_41cc_8246_e299c9060aa6"/>
        <hasMethod rdf:resource="Optional[http://www.semanticweb.org/team3/robo-ontology-0]/#turn_c551826f_033a_4c38_a61d_15a09c497816"/>
        <hasMethod rdf:resource="Optional[http://www.semanticweb.org/team3/robo-ontology-0]/#turn_d89c8822_ca9b_45b9_9336_d6c9331f06d5"/>
        <hasMethod rdf:resource="Optional[http://www.semanticweb.org/team3/robo-ontology-0]/#turn_eaaa623e_708d_442e_acc8_289e522c6c09"/>
        <hasMethod rdf:resource="Optional[http://www.semanticweb.org/team3/robo-ontology-0]/#turn_f6f73b8b_a875_4174_9790_6253db4c54fb"/>
    </owl:NamedIndividual>
    


    <!-- 
    ///////////////////////////////////////////////////////////////////////////////////////
    //
    // Annotations
    //
    ///////////////////////////////////////////////////////////////////////////////////////
     -->

    <rdf:Description rdf:about="http://www.semanticweb.org/team3/robo-ontology-0#Robo">
        <rdfs:label xml:lang="en">Robo</rdfs:label>
    </rdf:Description>
</rdf:RDF>



<!-- Generated by the OWL API (version 4.5.9.2019-02-01T07:24:44Z) https://github.com/owlcs/owlapi -->

